primeira parte de abs lemma principal

lambda_es.v
@@ -20,37 +20,11 @@ Proof.
     apply lt_le_trans with m; assumption.
 Qed.
 
-(* não utilizado
-Lemma in_or_notin: forall x s, x `in` s \/ x `notin` s.
-Proof.
-  intros. pose proof notin_diff_1. specialize (H x s s).
-  rewrite AtomSetProperties.diff_subset_equal in H.
-  - apply or_comm. apply H.
-    apply notin_empty_1.
-  - reflexivity.
-Qed. 
-
-Lemma remove_singleton_neq: forall x y,
-    x <> y -> remove y (singleton x) [=] singleton x.
-Proof.
-  intros. 
-  pose proof notin_singleton_2. specialize (H0 x y).
-  apply H0 in H.
-  apply AtomSetProperties.remove_equal in H. assumption.
-Qed. *)
-
 Lemma diff_remove_2: forall x y s,
   x <> y -> x `notin` remove y s -> x `notin` s.
 Proof.
   intros. default_simp.
 Qed. 
-
-(* não utilizado
-Lemma diff_equal: forall s s' t,
-    s [=] s' -> AtomSetImpl.diff s t [=] AtomSetImpl.diff s' t.
-Proof.
-intros. rewrite H. reflexivity.
-Qed. *)
 
 Lemma aux_not_equal : forall (x:atom) (y:atom),
     x <> y -> y <> x.
@@ -61,17 +35,6 @@ Proof.
   }
   contradiction.
 Qed.
-
-(* não utilizado 
-Lemma Sn_le_Sm__n_le_m : forall n m,
-  S n <= S m -> n <= m.
-Proof.
-  intros n m H. inversion H.
-  - apply le_n.
-  - apply (le_trans n (S n) m).
-    -- apply le_S. reflexivity.
-    -- assumption.
-Qed. *)
 
 Lemma remove_singleton_empty: forall x,
     remove x (singleton x) [=] empty.
@@ -153,24 +116,45 @@ Qed.
 
 (** * Introduction *)
 
-(** TBD  In this work, we present a formalization of an extension of the substitution lemma%\cite{barendregtLambdaCalculusIts1984}% with an explicit substitution operator in the Coq proof assistant%\cite{teamCoqProofAssistant2021}%. The substitution lemma is an important result concerning the composition of the substitution operation, and is usually presented as follows: if $x$ does not occur in the set of free variables of the term $v$ then $t\{x/u\}\{y/v\} =_\alpha t\{y/v\}\{x/u\{y/v\}\}$. This is a well known result already formalized several times in the context of the $\lambda$-calculus %\cite{berghoferHeadtoHeadComparisonBruijn2007}%.
+(** In this work, we present a formalization of the substitution lemma%\cite{barendregtLambdaCalculusIts1984}% in a general framework that extends the $\lambda$-calculus with an explicit substitution operator. The formalization is done in the Coq proof assistant%\cite{teamCoqProofAssistant2021}% and the source code is available at: %\vspace{0.25cm}%
 
-In the context of the $\lambda$-calculus with explicit substitutions its formalization is not straightforward because, in addition to the metasubstitution operation, there is the explicit substitution operator. Our formalization is done in a nominal setting that uses the MetaLib package of Coq, but no particular explicit substitution calculi is taken into account because the expected behaviour between the metasubstitution operation with the explicit substitutition constructor is the same regardless the calculus.
+ %\url{https://github.com/flaviodemoura/lx_confl/tree/m_subst_lemma} \vspace{0.25cm}%
 
-- This paper is written from a Coq script file.
-- include %\cite{berghoferHeadtoHeadComparisonBruijn2007}%
+The substitution lemma is an important result concerning the composition of the substitution operation, and is usually presented as follows in the context of the $\lambda$-calculus:
 
-*)
+%\begin{tcolorbox}
+ Let $t,u$ and $v$ be $\lambda$-terms. If $x\notin FV(v)$ ({\it i.e.} $x$ does not occur in the set of free variables of the term $v$) then $\metasub{\metasub{t}{x}{u}}{y}{v} =_\alpha \metasub{\metasub{t}{y}{v}}{x}{\metasub{u}{y}{v}}$.
+\end{tcolorbox}%
+
+This is a well known result already formalized in the context of the $\lambda$-calculus %\cite{berghoferHeadtoHeadComparisonBruijn2007}%. Nevertheless, in the context of $\lambda$-calculi with explicit substitutions its formalization is not straightforward due to the interaction between the metasubstitution and the explicit substitution operator. Our formalization is done in a nominal setting that uses the MetaLib%\footnote{\url{https://github.com/plclub/metalib}}% package of Coq, but no particular explicit substitution calculi is taken into account because the expected behaviour between the metasubstitution operation with the explicit substitutition constructor is the same regardless the calculus. The contributions of this work are twofold:
+
+%\begin{enumerate}
+\item The formalization is modular in the sense that no particular calculi with explicit substitutions is taken into account. Therefore, we believe that this formalization could be seen as a generic framework for proving properties of these calculi that uses the substitution lemma in the nominal setting\cite{kesnerPerpetualityFullSafe2008,nakazawaCompositionalConfluenceProofs2016,nakazawaPropertyShufflingCalculus2023};
+\item A solution to a circularity problem in the proofs is given. It adds an axiom to the formalization that replaces the set equality by the syntactic equality. In this way, we are allowed to replace/rewrite sets of (free) variables by another sets of (free) variables in arbitrary contexts.
+\end{enumerate}%
+
+This document is built directly from a Coq script using the CoqDoc%\footnote{\url{https://coq.inria.fr/refman/using/tools/coqdoc.html}}% tool. In the following section, we present the general framework and the basics of the nominal approach. In Section 3, we present our definition of metasubstitution and some of its properties. In Section 4, we present the main theorem, %{\it i.e.}% the substitution lemma, and we conclude in Section 5.*)
 
 (** * A syntactic extension of the $\lambda$-calculus *)
 
-(** In this section, we present the framework of the formalization, which is based on a nominal approach%\cite{gabbayNewApproachAbstract1999}% where variables use names instead of De Bruijn indexes%\cite{bruijnLambdaCalculusNotation1972}%. In the nominal setting, variables are represented by atoms that are structureless entities with a decidable equality: 
+(** In this section, we present the framework of the formalization, which is based on a nominal approach%\cite{gabbayNewApproachAbstract1999}% where variables use names. In the nominal setting, variables are represented by atoms that are structureless entities with a decidable equality: 
 
 <<
 Parameter eq_dec : forall x y : atom, {x = y} + {x <> y}.
 >>
 
-Variable renaming is done via name-swapping defined as follows:
+%\noindent% therefore different names mean different atoms and different variables. The nominal approach is close to the usual paper and pencil notation used in $\lambda$-calculus lectures, whose grammar of terms is given by:
+
+%\begin{equation}\label{lambda:grammar}
+ t ::= x \mid \lambda_x.t \mid t\ t
+\end{equation}%
+
+%\noindent% and its main rule, named $\beta$-reduction, is given by:
+
+%\begin{equation}\label{lambda:beta}
+ (\lambda_x.t)\ u \to_{\beta} \metasub{t}{x}{u}
+\end{equation}%
+%\noindent% where $\metasub{t}{x}{u}$ represents the term obtained from $t$ after replacing all its free occurrences of the variable $x$ by $u$ in a way that renaming of bound variable is done in order to avoid variable capture. In other words, $\metasub{t}{x}{u}$ is a metanotation for a capture free substitution. For instance, the $\lambda$-term $(\lambda_x\lambda_y.x\ y)\ y$ has both bound and free occurrences of the variable $y$. In order to $\beta$-reduce it one has to replace (or substitute) the free variable $y$ for all free occurrences of the variable $x$ in the term $(\lambda_y.x\ y)$. But a straight substitution will capture the free variable $y$, %{\it i.e.}% this means that the free occurrence of $y$ before the $\beta$-reduction will become bound after the $\beta$-reduction step. A renaming of bound variables is done to avoid such capture, so in this example, one can take an $\alpha$-equivalent%\footnote{A formal definition of this notion will be given later in this section.}% term, say $(\lambda_z.x\ z)$, and perform the $\beta$-step correctly as $(\lambda_x\lambda_y.x\ y)\ y \to_{\beta} \lambda_z.y\ z$. The renaming of variables in the nominal setting is done via a name-swapping, which is formally defined as follows:
 
 $\vswap{x}{y}{z} := \left\{ \begin{array}{ll}
 y, & \mbox{ if } z = x; \\
@@ -178,13 +162,19 @@ x, & \mbox{ if } z = y; \\
 z, & \mbox{ otherwise. } \\
 \end{array}\right.$
 
-\noindent and the corresponding Coq definition:
+This notion can be extended to $\lambda$-terms in a straightfoward way:
 
- *)
+$\swap{x}{y}{t} := \left\{ \begin{array}{ll}
+\vswap{x}{y}{z}, & \mbox{ if } t = z; \\
+\lambda_{\vswap{x}{y}{z}}.\swap{x}{y}{t_1}, & \mbox{ if } t = \lambda_z.t_1; \\
+\swap{x}{y}{t_1}\ \swap{x}{y}{t_2}, & \mbox{ if } t = t_1\ t_2\\
+\end{array}\right.$
 
-Definition swap_var (x:atom) (y:atom) (z:atom) :=
-  if (z == x) then y else if (z == y) then x else z.
+In the previous example, one could apply a swap to avoid the variable capture in the following way: $(\lambda_x\lambda_y.x\ y)\ y \to_{\beta} \metasub{\swap{x}{z}{(\lambda_y.x\ y)}}{x}{y} = \lambda_z.y\ z$. Could we have used a variable substitution instead of a swapping in the previous example? Sure! We could have done the reduction as $(\lambda_x\lambda_y.x\ y)\ y \to_{\beta} \metasub{\metasub{(\lambda_y.x\ y)}}{x}{y}{x}{z} = \lambda_z.y\ z$, but as we will see soon, variable substitution is not stable under $\alpha$-equivalence, and this stability property is necessary to work modulo $\alpha$-equivalence.
 
+In what follows, we will interleave metanotation with the corresponding Coq notation because this strategy will be better for explaining the proof steps of the forthcoming lemmas. So the swapping of variables, named [swap_var], is defined as follows: *)
+
+Definition swap_var (x:atom) (y:atom) (z:atom) := if (z == x) then y else if (z == y) then x else z.
 
 (* begin hide *)
 Lemma swap_var_id: forall x y, (swap_var x x y = y).
@@ -193,7 +183,7 @@ Proof.
 Qed.
 (* end hide *)
 
-(** The next step is to extend the variable renaming operation to terms, which in our case corresponds to $\lambda$-terms augmented with an explicit substitution operation given by the following inductive grammar: *)
+(** The next step is to extend the variable renaming operation to terms, which in our case corresponds to $\lambda$-terms augmented with an explicit substitution operation. We use [n_sexp] to denote the set of nominal expressions equipped with an explicit substitution operator, which, for simplicity, we will refer to as just "terms", and the corresponding grammar is outlined below: *)
 
 Inductive n_sexp : Set :=
  | n_var (x:atom)
@@ -201,20 +191,8 @@ Inductive n_sexp : Set :=
  | n_app (t1:n_sexp) (t2:n_sexp)
  | n_sub (t1:n_sexp) (x:atom) (t2:n_sexp).
 
-(** %\noindent% where [n_var] is the constructor for variables, [n_abs] for abstractions, [n_app] for applications and [n_sub] for the explicit substitution operation. Explicit substitution calculi are formalisms that decompose the metasubstitution operation into more atomic steps behaving as a bridge between the $\lambda$-calculus and its implementations. In other words, explicit substitution calculi "allow a better understanding of the execution models of higher-order languages"%\cite{kesnerTheoryExplicitSubstitutions2009}%. The action of a permutation on a term, written $\swap{x}{y}{t}$, is inductively defined as follows:%\vspace{.5cm}%
+(** %\noindent% where [n_var] is the constructor for variables, [n_abs] for abstractions, [n_app] for applications and [n_sub] for the explicit substitution. Explicit substitution calculi are formalisms that deconstruct the metasubstitution operation into more granular steps, thereby functioning as an intermediary between the $\lambda$-calculus and its practical implementations. In other words, these calculi shed light on the execution models of higher-order languages%\cite{kesnerTheoryExplicitSubstitutions2009}%. The [size] of terms and the set [fv_nom] of the free variables of a term are defined as usual: *)
 
-$\swap{x}{y}{t} := \left\{ \begin{array}{ll}
-\vswap{x}{y}{v}, & \mbox{ if } t \mbox{ is the variable } v; \\
-\lambda_{\vswap{x}{y}{z}}. \swap{x}{y}{t_1}, & \mbox{ if } t = \lambda_z.t_1; \\
-\swap{x}{y}{t_1}\ \swap{x}{y}{t_2}, & \mbox{ if } t = t_1\ t_2;\\
-\swap{x}{y}{t_1}[\vswap{x}{y}{z} := \swap{x}{y}{t_2}], & \mbox{ if } t = t_1[z := t_2].
-\end{array}\right.$%\vspace{.5cm}%
-
-The corresponding Coq definition is given by the following recursive function:
-
- *)
-
-(* begin hide *)
 Fixpoint size (t : n_sexp) : nat :=
   match t with
   | n_var x => 1
@@ -223,14 +201,24 @@ Fixpoint size (t : n_sexp) : nat :=
   | n_sub t1 x t2 => 1 + size t1 + size t2
   end.
 
-Fixpoint fv_nom (n : n_sexp) : atoms :=
-  match n with
+Fixpoint fv_nom (t : n_sexp) : atoms :=
+  match t with
   | n_var x => {{x}}
-  | n_abs x n => remove x (fv_nom n)
+  | n_abs x t1 => remove x (fv_nom t1)
   | n_app t1 t2 => fv_nom t1 `union` fv_nom t2
   | n_sub t1 x t2 => (remove x (fv_nom t1)) `union` fv_nom t2
   end.
-(* end hide *)
+
+(** The action of a permutation on a term, written $\swap{x}{y}{t}$, is inductively defined as follows:%\vspace{.5cm}%
+
+$\swap{x}{y}{t} := \left\{ \begin{array}{ll}
+\vswap{x}{y}{v}, & \mbox{ if } t \mbox{ is the variable } v; \\
+\lambda_{\vswap{x}{y}{z}}. \swap{x}{y}{t_1}, & \mbox{ if } t = \lambda_z.t_1; \\
+\swap{x}{y}{t_1}\ \swap{x}{y}{t_2}, & \mbox{ if } t = t_1\ t_2;\\
+\esub{\swap{x}{y}{t_1}}{\vswap{x}{y}{z}}{\swap{x}{y}{t_2}}, & \mbox{ if } t = \esub{t_1}{z}{t_2}.
+\end{array}\right.$ %\vspace{.5cm}%
+
+The corresponding Coq definition is given by the following recursive function: *)
 
 Fixpoint swap (x:atom) (y:atom) (t:n_sexp) : n_sexp :=
   match t with
@@ -239,8 +227,6 @@ Fixpoint swap (x:atom) (y:atom) (t:n_sexp) : n_sexp :=
   | n_app t1 t2 => n_app (swap x y t1) (swap x y t2)
   | n_sub t1 z t2 => n_sub (swap x y t1) (swap_var x y z) (swap x y t2)
   end.
-
-(** The key point of this approach is that the swap opearation ... *)
 
 (* begin hide *)
 Lemma swap_id : forall t x,
@@ -276,68 +262,16 @@ Proof.
   - subst. apply swap_eq in H2. contradiction.
   - apply swap_eq in H2. contradiction.
 Qed.
-  
-Lemma swap_size_eq : forall x y t,
-    size (swap x y t) = size t.
+(* end hide *)
+
+(** The [swap] function preserves the size of terms, as stated by the following lemma: *)
+Lemma swap_size_eq : forall x y t, size (swap x y t) = size t.
 Proof.
   induction t; simpl; auto.
 Qed.
 
+(* begin hide *)
 Hint Rewrite swap_size_eq.
-
-Lemma n_sexp_induction :
- forall P : n_sexp -> Prop,
- (forall x, P (n_var x)) ->
- (forall t1 z,
-    (forall t2 x y, size t2 = size t1 ->
-    P (swap x y t2)) -> P (n_abs z t1)) ->
- (forall t1 t2, P t1 -> P t2 -> P (n_app t1 t2)) ->
- (forall t1 t3 z, P t3 -> 
-    (forall t2 x y, size t2 = size t1 ->
-    P (swap x y t2)) -> P (n_sub t1 z t3)) -> 
- (forall t, P t).
-Proof.
-  intros P Hvar Habs Happ Hsub t.
-  remember (size t) as n.
-  generalize dependent t.
-  induction n using strong_induction.
-  intro t; case t.
-  - intros x Hsize.
-    apply Hvar.
-  - intros x t' Hsize.
-    apply Habs.
-    intros t'' x1 x2 Hsize'.
-    apply H with (size t'').
-    + rewrite Hsize'.
-      rewrite Hsize.
-      simpl.
-      apply Nat.lt_succ_diag_r.
-    + symmetry.
-      apply swap_size_eq.
-  - intros. apply Happ.
-    + apply H with ((size t1)).
-      ++ simpl in Heqn. rewrite Heqn.
-         apply le_lt_n_Sm.
-         apply le_plus_l.
-      ++ reflexivity.
-    + apply H with ((size t2)).
-      ++ simpl in Heqn. rewrite Heqn.
-          apply le_lt_n_Sm.
-         apply le_plus_r.
-      ++ reflexivity.
-  - intros. apply Hsub.
-    + apply H with ((size t2)).
-      ++ simpl in Heqn. rewrite Heqn.
-          apply le_lt_n_Sm.
-         apply le_plus_r.
-      ++ reflexivity.
-    + intros. apply H with ((size (swap x0 y t0))).
-      ++ rewrite swap_size_eq. rewrite H0.
-         simpl in Heqn. rewrite Heqn.
-         apply le_lt_n_Sm.
-         apply le_plus_l.
-      ++ reflexivity.
-Qed. 
 
 Lemma swap_symmetric : forall t x y, swap x y t = swap y x t.
 Proof.
@@ -366,7 +300,6 @@ Lemma shuffle_swap : forall w y n z,
 Proof.
   induction n; intros; simpl; unfold swap_var; default_simp.
 Qed.
-(* end hide *)
 
 Lemma shuffle_swap' : forall w y n z,
     w <> z -> y <> z ->
@@ -374,7 +307,9 @@ Lemma shuffle_swap' : forall w y n z,
 Proof.
   induction n; intros; simpl; unfold swap_var; default_simp.
 Qed.
+(* end hide *)
 
+(** Equivariance is an important property of swap:*)
 Lemma swap_var_equivariance : forall v x y z w,
     swap_var x y (swap_var z w v) =
     swap_var (swap_var x y z) (swap_var x y w) (swap_var x y v).
@@ -382,7 +317,6 @@ Proof.
   intros; unfold swap_var; case(v == z); case (w == x); default_simp.
 Qed.
 
-(* begin hide *)
 Lemma swap_equivariance : forall t x y z w,
     swap x y (swap z w t) = swap (swap_var x y z) (swap_var x y w) (swap x y t).
 Proof.
@@ -406,7 +340,7 @@ Proof.
   - intros. simpl. rewrite IHt1. rewrite IHt2. unfold swap_var.
     default_simp.    
 Qed.
-
+(* begin hide *)
 Lemma fv_nom_swap : forall z y t,
   z `notin` fv_nom t ->
   y `notin` fv_nom (swap y z t).
@@ -452,280 +386,7 @@ Proof.
        --- assumption.
        --- assumption.
 Qed. 
-(* end hide *)
 
-
-(* não utilizado
-Lemma in_fv_nom_equivariance : forall x y x0 t,
-  x0 `in` fv_nom t ->
-  swap_var x y x0 `in` fv_nom (swap x y t).
-Proof.
-  induction t.
-  - simpl. intro H. pose proof singleton_iff.
-    specialize (H0 x1 x0). apply H0 in H. rewrite H.
-    apply singleton_iff. reflexivity.
-  - simpl. intros. unfold swap_var. default_simp.
-    -- pose proof AtomSetImpl.remove_1.
-       assert (H1:x `notin` remove x (fv_nom t)). {
-         apply H0. reflexivity.
-       }contradiction.
-    -- pose proof AtomSetImpl.remove_2. apply H0.
-       --- unfold not. intro. symmetry in H1. contradiction.
-       --- specialize (H0 (fv_nom t) y x). assert(y<>x). {
-             apply n.
-           }
-           
-           apply H0 in n.
-           + apply AtomSetImpl.remove_3 in H. apply IHt in H.
-             unfold swap_var in IHt. case (x == x) in IHt.
-             ++ apply AtomSetImpl.remove_3 in n.
-                apply IHt in n. assumption.
-             ++ unfold not in n0. contradiction. 
-           + apply AtomSetImpl.remove_3 in H. assumption.
-    -- apply AtomSetImpl.remove_2.
-       --- assumption.
-       --- apply AtomSetImpl.remove_3 in H. apply IHt in H.
-           unfold swap_var in H. case (x == x) in H.
-           + assumption.
-           + contradiction.
-    -- apply AtomSetImpl.remove_2.
-       --- assumption.
-       --- apply AtomSetImpl.remove_3 in H. unfold swap_var in IHt.
-           case (y == x) in IHt.
-           + intros. contradiction.
-           + intros. case (y == y) in IHt.
-             ++ apply IHt in H. assumption.
-             ++ contradiction.
-    -- assert (y = y). {
-         reflexivity.
-       }
-       pose proof AtomSetImpl.remove_1.
-       specialize (H1 (fv_nom t) y y).
-       apply H1 in H0. unfold not in H0. contradiction.
-    -- unfold swap_var in IHt. case (y == x) in IHt.
-       --- contradiction.
-       --- case (y == y) in IHt.
-           + apply AtomSetImpl.remove_3 in H. apply IHt in H.
-             pose proof AtomSetImpl.remove_2.
-             specialize (H0 (fv_nom (swap x y t)) x1 x).
-             apply H0 in n0.
-             ++ assumption.
-             ++ assumption.
-           + contradiction.
-    -- apply AtomSetImpl.remove_3 in H. apply IHt in H.
-       unfold swap_var in H. case(x0 == x) in H.
-       --- contradiction.
-       --- case(x0 == y) in H.
-           + pose proof AtomSetImpl.remove_2.
-             specialize (H0 (fv_nom (swap x y t)) y x0).
-             apply aux_not_equal in n0. apply H0 in n0.
-             ++ assumption.
-             ++ symmetry in e. contradiction.
-           + unfold swap_var in IHt. case (x0 == x) in IHt.
-             ++ contradiction.
-             ++ pose proof AtomSetImpl.remove_2.
-                specialize (H0 (fv_nom (swap x y t)) y x0).
-                apply aux_not_equal in n0. apply H0 in n0.
-                +++ assumption.
-                +++ assumption.
-    -- unfold swap_var in IHt. default_simp.
-       apply AtomSetImpl.remove_3 in H. apply IHt in H.
-       pose proof AtomSetImpl.remove_2.
-       specialize (H0 (fv_nom (swap x y t)) x x0).
-       apply aux_not_equal in n. apply H0 in n.
-       --- assumption.
-       --- assumption.
-    -- case (x == y). 
-       --- intros. rewrite e. rewrite swap_id. assumption.
-       --- intros. case (x0 == x1).
-           + intros. rewrite e in H. pose proof notin_remove_3.
-             specialize (H0 x1 x1 (fv_nom t)). assert (x1 = x1). {
-               reflexivity.
-             }
-             apply H0 in H1. unfold not in H1. contradiction.
-           + intros. apply AtomSetImpl.remove_3 in H.
-             unfold swap_var in IHt. case (x0 == x) in IHt.
-             ++ contradiction.
-             ++ case (x0 == y) in IHt.
-                +++ contradiction.
-                +++ apply IHt in H. pose proof remove_neq_iff.
-                    specialize (H0 (fv_nom (swap x y t)) x1 x0).
-                    apply aux_not_equal in n4.
-                    apply H0 in n4. apply n4 in H. assumption.      
-  - unfold swap_var. unfold swap_var in IHt1.
-    unfold swap_var in IHt2. default_simp.
-    -- pose proof AtomSetImpl.union_1.
-       specialize (H0 (fv_nom t1) (fv_nom t2) x). apply H0 in H.
-       pose proof AtomSetImpl.union_2.
-       inversion H. 
-       --- specialize (H1 (fv_nom (swap x y t1)) (fv_nom (swap x y t2)) y). apply IHt1 in H2.  apply H1 in H2. assumption.
-       --- specialize (H1 (fv_nom (swap x y t2)) (fv_nom (swap x y t1)) y).
-           pose proof AtomSetProperties.union_sym. apply H3.
-           apply IHt2 in H2.  apply H1 in H2. assumption.
-    -- pose proof union_iff. apply union_iff in H. inversion H.
-       --- apply IHt1 in H1. apply union_iff. left. assumption.
-       --- apply IHt2 in H1. apply union_iff. right. assumption.
-    -- apply union_iff in H. inversion H.
-       --- apply union_iff. apply IHt1 in H0. left. assumption.
-       --- apply union_iff. apply IHt2 in H0. right. assumption.
-  - intros. simpl. unfold swap_var. case (x == y).
-    -- intros. default_simp.
-       --- repeat rewrite swap_id. assumption.
-       --- repeat rewrite swap_id. assumption.
-       --- repeat rewrite swap_id. assumption.
-       --- repeat rewrite swap_id. assumption.
-    -- intros. default_simp.
-       --- pose proof AtomSetImpl.remove_1.
-           specialize (H0 (fv_nom t1) x x).
-           assert (x = x). {
-             reflexivity.
-           }
-           apply H0 in H1. pose proof union_iff. apply H2.
-           apply H2 in H. inversion H.
-           + contradiction.
-           + right. simpl. apply IHt2 in H3. unfold swap_var in H3.
-             case (x == x) in H3.
-             ++ assumption.
-             ++ contradiction.
-       --- apply union_iff in H. apply union_iff. inversion H.
-           + unfold swap_var in IHt2. case (x == x) in IHt2.
-             ++ apply remove_iff in H0. inversion H0.
-                unfold swap_var in IHt1. case (x == x) in IHt1.
-                +++ apply IHt1 in H1. pose proof remove_neq_iff.
-                    left. apply H3.
-                    * assumption.
-                    * assumption.                
-                +++ contradiction.
-             ++ contradiction.
-           + apply IHt2 in H0. unfold swap_var in H0.
-             case (x == x) in H0.
-             ++ right. assumption.
-             ++ contradiction.
-       --- apply union_iff. apply union_iff in H. inversion H.
-           + apply remove_neq_iff in H0. apply IHt1 in H0.
-             unfold swap_var in H0. case (x == x) in H0.
-             ++ left. apply remove_iff. split.
-                +++ assumption.
-                +++ assumption.
-             ++ contradiction.
-             ++ assumption.
-           + apply IHt2 in H0. unfold swap_var in H0.
-             case (x == x) in H0.
-             ++ right. assumption.
-             ++ contradiction.
-       --- apply union_iff. apply union_iff in H. inversion H.
-           + apply remove_neq_iff in H0. apply IHt1 in H0.
-             unfold swap_var in H0. case (y == x) in H0.
-             ++ contradiction.
-             ++ case (y == y) in H0.
-                +++ left. apply remove_iff. split.
-                    * assumption.
-                    * assumption.
-                +++ contradiction.
-             ++ assumption.
-           + apply IHt2 in H0. unfold swap_var in H0.
-             case (y == x) in H0.
-             ++ contradiction.
-             ++ case (y == y) in H0.
-                +++ right. assumption.
-                +++ contradiction.
-       --- pose proof AtomSetImpl.remove_1.
-           specialize (H0 (fv_nom t1) x x).
-           assert (x = x). {
-             reflexivity.
-           }
-           apply H0 in H1. apply union_iff. right.
-           unfold swap_var in IHt2. case (y == x) in IHt2.
-           + contradiction.
-           + case (y == y) in IHt2.
-             ++ apply union_iff in H. inversion H.
-                +++ pose proof AtomSetImpl.remove_1.
-                    specialize (H3 (fv_nom t1) y y).
-                    assert (y = y). {
-                      reflexivity.
-                    }
-                    apply H3 in H4. contradiction.
-                +++ apply IHt2 in H2. assumption.
-             ++ contradiction.
-       --- apply union_iff. apply union_iff in H. inversion H.
-           + apply remove_neq_iff in H0. apply IHt1 in H0.
-             unfold swap_var in H0. case (y == x) in H0.
-             ++ contradiction.
-             ++ case (y == y) in H0.
-                +++ left. apply remove_neq_iff.
-                    * assumption.
-                    * assumption.
-                +++ contradiction.
-             ++ assumption.  
-           + apply IHt2 in H0. unfold swap_var in H0.
-             case (y == x) in H0.
-             ++ contradiction.
-             ++ case (y == y) in H0.
-                +++ right. assumption.
-                +++ contradiction.
-       --- apply union_iff. apply union_iff in H. inversion H.
-           + apply remove_neq_iff in H0. apply IHt1 in H0.
-             unfold swap_var in H0. case (x0 == x) in H0.
-             ++ contradiction.
-             ++ case (x0 == y) in H0.
-                +++ contradiction.
-                +++ left. apply remove_neq_iff.
-                    * apply aux_not_equal. assumption.
-                    * assumption.
-             ++ apply aux_not_equal. assumption.  
-           + apply IHt2 in H0. unfold swap_var in H0.
-             case (x0 == x) in H0.
-             ++ contradiction.
-             ++ case (x0 == y) in H0.
-                +++ contradiction.
-                +++ right. assumption. 
-       --- apply union_iff. apply union_iff in H. inversion H.
-           + apply remove_neq_iff in H0.
-             ++ apply IHt1 in H0. unfold swap_var in H0.
-                case (x0 == x) in H0.
-                +++ contradiction.
-                +++ case (x0 == y) in H0.
-                    * contradiction.
-                    * left. apply remove_neq_iff.
-                      ** apply aux_not_equal. assumption.
-                      ** assumption.
-             ++ apply aux_not_equal. assumption.
-           + apply IHt2 in H0. unfold swap_var in H0.
-             case (x0 == x) in H0.
-             ++ contradiction.
-             ++ case (x0 == y) in H0.
-                +++ contradiction.
-                +++ right. assumption.
-       --- apply union_iff. apply union_iff in H. case (x1 == x0).
-           + intros. right. inversion H.
-             ++ rewrite e in H0. apply remove_iff in H0.
-                inversion H0. contradiction.
-             ++ apply IHt2 in H0. unfold swap_var in H0.
-                case (x0 == x) in H0.
-                +++ contradiction.
-                +++ case (x0 == y) in H0.
-                    * contradiction.
-                    * assumption.
-           + inversion H.
-             ++ intros. apply remove_neq_iff in H0.
-                +++ apply IHt1 in H0. unfold swap_var in H0.
-                case (x0 == x) in H0.
-                    * contradiction.
-                    * case (x0 == y) in H0.
-                      ** contradiction.
-                      ** left. apply remove_neq_iff.
-                         *** assumption.
-                         *** assumption.
-                +++ assumption.
-             ++ intros. apply IHt2 in H0. unfold swap_var in H0.
-                case (x0 == x) in H0.
-                +++ contradiction.
-                +++ case (x0 == y) in H0.
-                    * contradiction.
-                    * right. assumption.
-Qed.*)
-
-(* begin hide *)
 Lemma swap_remove_reduction: forall x y t,
     remove x (remove y (fv_nom (swap y x t))) [=] remove x (remove y (fv_nom t)).
 Proof.
@@ -788,8 +449,7 @@ Proof.
 Qed.
 
 Lemma remove_fv_swap: forall x y t, x `notin` fv_nom t -> remove x (fv_nom (swap y x t)) [=] remove y (fv_nom t).
-Proof.
-  (** %\noindent {\bf Proof.}% The proof is by induction on the structure of [t].%\newline% *)
+Proof. (** %\noindent {\bf Proof.}% The proof is by induction on the structure of [t].%\newline% *)
   intros x y t. induction t.
   (** %\noindent%$\bullet$ The first case is when [t] is a variable, say [x0]. By hypothesis [x0 <> x], and we need to show that [remove x (fv_nom (swap y x x0)) [=] remove y (fv_nom x0)]. There are two cases to consider: *)
   - intro Hfv. simpl in *. apply notin_singleton_1 in Hfv. unfold swap_var. case (x0 == y).
@@ -831,7 +491,7 @@ Proof.
     + unfold swap_var. case (x0 == y); intros; subst.
       unfold swap_var in H1. rewrite eq_dec_refl in H1. rewrite double_remove in *. apply IHt2 in Hfv. case (x == y); intros; subst.
       * repeat rewrite swap_id in *. rewrite double_remove. reflexivity.
-      * rewrite double_remove. apply IHt1. Search remove. apply diff_remove_2 in Hfv'.
+      * rewrite double_remove. apply IHt1. apply diff_remove_2 in Hfv'.
         ** assumption.
         ** assumption.
       * destruct (x0 == x).
@@ -840,111 +500,52 @@ Proof.
            {
            rewrite remove_symmetric. reflexivity.
            }
-           rewrite Hr. clear Hr. apply AtomSetProperties.Equal_remove. apply IHt1. Search remove. apply diff_remove_2 in Hfv'.
+           rewrite Hr. clear Hr. apply AtomSetProperties.Equal_remove. apply IHt1. apply diff_remove_2 in Hfv'.
             *** assumption.
             *** auto.
     + apply IHt2. apply Hfv.
 Qed.
 (* end hide *)
 
-(*        subst. repeat rewrite double_remove. rewrite swap_id. reflexivity.
-      * repeat rewrite double_remove. apply IHt. assumption.
-    + intro Hneq. case (x0 == x).
-      * intro Heq. subst. rewrite swap_remove_reduction. rewrite remove_symmetric. reflexivity.
-      * intro Hneq'. rewrite remove_symmetric. symmetry. rewrite remove_symmetric. symmetry.
-        apply AtomSetProperties.Equal_remove. apply IHt. simpl in Hfv. apply notin_remove_1 in Hfv. inversion Hfv.
-        ** contradiction.
-        ** assumption.           
-  - intro Hfv. simpl in *. pose proof Hfv as Hfv'. apply notin_union_1 in Hfv'. apply notin_union_2 in Hfv.
-    apply IHt1 in Hfv'. apply IHt2 in Hfv. pose proof remove_union_distrib as H1. pose proof H1 as H2.
-    specialize (H1 (fv_nom (swap y x t1)) (fv_nom (swap y x t2)) x). specialize (H2 (fv_nom t1) (fv_nom t2) y). rewrite Hfv' in H1. rewrite Hfv in H1. rewrite H1. rewrite H2. reflexivity.
-  - intro Hfv. simpl in *. pose proof Hfv as Hfv'. apply notin_union_1 in Hfv'. apply notin_union_2 in Hfv.
-    pose proof remove_union_distrib as H1. pose proof H1 as H2.
-    specialize (H1 (remove (swap_var y x x0) (fv_nom (swap y x t1))) (fv_nom (swap y x t2)) x). rewrite H1.
-    specialize (H2 (remove x0 (fv_nom t1)) (fv_nom t2) y). rewrite H2. apply Equal_union_compat.
-    + unfold swap_var. case (x0 == y); intros; subst.
-      unfold swap_var in H1. rewrite eq_dec_refl in H1. rewrite double_remove in *. apply IHt2 in Hfv. case (x == y); intros; subst.
-      * repeat rewrite swap_id in *. Admitted. *)
+(** The notion of $\alpha$-equivalence is defined in the usual way by the following rules:
 
-(*        
-        reflexivity.
-      * apply notin_remove_1 in Hfv'. inversion Hfv'; subst.
-        ** contradiction.
-        ** clear Hfv'. pose proof remove_union_distrib as H3. pose proof H3 as H4.
-           specialize (H3 (remove y (fv_nom t1)) (fv_nom (swap y x t2)) x).
-           specialize (H4 (remove y (fv_nom t1)) (fv_nom t2) y). rewrite H1. rewrite H2. rewrite double_remove in H4.
-           apply diff_remove with x y (fv_nom t1) in n.
-           *** apply AtomSetProperties.remove_equal in n.
+%\begin{mathpar}
+ \inferrule*[Right={({\rm\it aeq\_var})}]{~}{x =_\alpha x} \and  \inferrule*[Right={({\rm\it aeq\_abs\_same})}]{t_1 =_\alpha t_2}{\lambda_x.t_1 =_\alpha \lambda_x.t_2} 
+\end{mathpar}%
 
+%\begin{mathpar}
+\inferrule*[Right={({\rm\it aeq\_abs\_diff})}]{x \neq y \and x \notin fv(t_2) \and t_1 =_\alpha \swap{y}{x}{t_2}}{\lambda_x.t_1 =_\alpha \lambda_y.t_2} 
+\end{mathpar}%
 
+%\begin{mathpar}
+ \inferrule*[Right={({\rm\it aeq\_app})}]{t_1 =_\alpha t_1' \and t_2 =_\alpha t_2'}{t_1\ t_2 =_\alpha t_1'\ t_2'} \and  \inferrule*[Right={({\rm\it aeq\_sub\_same})}]{t_1 =_\alpha t_1' \and t_2 =_\alpha t_2'}{\esub{t_1}{x}{t_2} =_\alpha \esub{t_1'}{x}{t_2'}} 
+\end{mathpar}%
 
-               rewrite H2 in H4.
-               rewrite n in H4; rewrite H4; rewrite H5.
-                      reflexivity.
-           *** assumption.
-       --- contradiction.
-  -- case (x0 == x); intros; subst.
-     --- unfold swap_var in H0. case (x == y) in H0; intros.
-         + contradiction.
-         + case (x == x) in H0; intros.
-           ++ simpl in H. pose proof H. apply notin_union_1 in H.
-              apply notin_union_2 in H2. apply IHt2 in H2.
-              rewrite H2 in H0. symmetry. Search "remove_union".
-              rewrite remove_union_distrib. symmetry.
-              rewrite remove_symmetric.
-              rewrite swap_remove_reduction in H0. assumption.
-           ++ contradiction.
-     --- simpl in H. pose proof H. apply notin_union_1 in H.
-         apply notin_remove_1 in H. inversion H; subst.
-         + contradiction.
-         + apply notin_union_2 in H2.
-           apply IHt1 in H3; apply IHt2 in H2.
-           unfold swap_var in H0. default_simp.
-           rewrite H0. rewrite remove_symmetric.
-           rewrite H1; rewrite H2; rewrite H3.
-           rewrite remove_symmetric. reflexivity.        
-Qed.*)
+%\begin{mathpar}
+\inferrule*[Right={({\rm\it aeq\_sub\_diff})}]{t_2 =_\alpha t_2' \and x \neq y \and x \notin fv(t_1') \and t_1 =_\alpha \swap{y}{x}{t_1'}}{\esub{t_1}{x}{t_2} =_\alpha \esub{t_1'}{y}{t_2'}} 
+\end{mathpar}%
 
-(* ver necessidade
-Lemma fv_nom_swap_eq: forall x y t, x `notin` fv_nom t -> y `notin` fv_nom t -> fv_nom t [=] fv_nom (swap x y t).
-Proof.
-  induction t using n_sexp_induction.
-  - intros H1 H2. simpl in *.
-    unfold swap_var. default_simp.
-    + apply notin_singleton_is_false in H1. contradiction.
-    + apply notin_singleton_is_false in H2. contradiction.     
-    + reflexivity.
-  - intros H1 H2. simpl in *.
-    Admitted. *)
-
-(** The notion of $\alpha$-equivalence is defined as follows: *)
+Each of these rules correspond to a constructor in the [aeq] inductive definition below: *)
 
 Inductive aeq : n_sexp -> n_sexp -> Prop :=
- | aeq_var : forall x,
-     aeq (n_var x) (n_var x)
- | aeq_abs_same : forall x t1 t2,
-     aeq t1 t2 -> aeq (n_abs x t1) (n_abs x t2)
- | aeq_abs_diff : forall x y t1 t2,
-     x <> y -> x `notin` fv_nom t2 ->
-     aeq t1 (swap y x t2) ->
-     aeq (n_abs x t1) (n_abs y t2)
- | aeq_app : forall t1 t2 t1' t2',
-     aeq t1 t1' -> aeq t2 t2' ->
-     aeq (n_app t1 t2) (n_app t1' t2')
- | aeq_sub_same : forall t1 t2 t1' t2' x,
-     aeq t1 t1' -> aeq t2 t2' ->
-     aeq (n_sub t1 x t2) (n_sub t1' x t2')
- | aeq_sub_diff : forall t1 t2 t1' t2' x y,
-     aeq t2 t2' -> x <> y -> x `notin` fv_nom t1' ->
-     aeq t1 (swap y x t1') ->
-     aeq (n_sub t1 x t2) (n_sub t1' y t2').
-
-(** %\noindent% where ... *)
-
+| aeq_var : forall x, aeq (n_var x) (n_var x)
+| aeq_abs_same : forall x t1 t2, aeq t1 t2 -> aeq (n_abs x t1)(n_abs x t2)
+| aeq_abs_diff : forall x y t1 t2, x <> y -> x `notin` fv_nom t2 -> aeq t1 (swap y x t2) -> aeq (n_abs x t1) (n_abs y t2)
+| aeq_app : forall t1 t2 t1' t2', aeq t1 t1' -> aeq t2 t2' -> aeq (n_app t1 t2) (n_app t1' t2')
+| aeq_sub_same : forall t1 t2 t1' t2' x, aeq t1 t1' -> aeq t2 t2' -> aeq (n_sub t1 x t2) (n_sub t1' x t2')
+| aeq_sub_diff : forall t1 t2 t1' t2' x y, aeq t2 t2' -> x <> y -> x `notin` fv_nom t1' -> aeq t1 (swap y x t1') -> aeq (n_sub t1 x t2) (n_sub t1' y t2').
 (* begin hide *)
 Hint Constructors aeq.
-Notation "t =a u" := (aeq t u) (at level 60).
+(* end hide *)
 
+(** In what follows, we use a infix notation for $\alpha$-equivalence in the Coq code: we write [t =a u] instead of [aeq t u]. *)
+
+(* begin hide *)
+Notation "t =a u" := (aeq t u) (at level 60).
+(* end hide *)
+
+(** The above notion defines an equivalence relation over the set [n_sexp] of nominal expressions with explicit substitutions, %{\it i.e.}% the [aeq] relation is reflexive, symmetric and transitive. *)
+(* begin hide *)
 Example aeq1 : forall x y, x <> y -> (n_abs x (n_var x)) =a (n_abs y (n_var y)).
 Proof.
   intros.
@@ -956,6 +557,9 @@ Lemma aeq_var_2 : forall x y, (n_var x) =a (n_var y) -> x = y.
 Proof.
   intros. inversion H; subst. reflexivity.
 Qed.
+(* end hide *)
+
+(** Informally, two terms are $\alpha$-equivalent if they differ only by the names of the bound variables. Therefore, $\alpha$-equivalent terms have the same size, and the same set of free variables: *)
 
 Lemma aeq_size: forall t1 t2, t1 =a t2 -> size t1 = size t2.
 Proof.
@@ -967,13 +571,6 @@ Proof.
   - simpl. rewrite IHaeq1. rewrite IHaeq2. reflexivity.
   - simpl. rewrite IHaeq1. rewrite IHaeq2. rewrite swap_size_eq. reflexivity.
 Qed.
-
-Lemma aeq_refl : forall n, n =a n.
-Proof.
-  induction n; auto.
-Qed.
-(* end hide *)
-
 Lemma aeq_fv_nom : forall t1 t2, t1 =a t2 -> fv_nom t1 [=] fv_nom t2.
 Proof.
   intros. induction H.
@@ -986,6 +583,11 @@ Proof.
     specialize (H3 x y t1'). apply H3 in H1.
     inversion H2; subst; rewrite IHaeq1; rewrite IHaeq2; rewrite H1; reflexivity.
 Qed.  
+(* begin hide *)
+Lemma aeq_refl : forall n, n =a n.
+Proof.
+  induction n; auto.
+Qed.
 
 Lemma aeq_swap1: forall t1 t2 x y, t1 =a t2 -> (swap x y t1) =a (swap x y t2).
 Proof.
@@ -1456,6 +1058,34 @@ Proof.
                 +++ apply aux_not_equal; assumption.
 Qed.
 
+Lemma aeq_sym: forall t1 t2, t1 =a t2 -> t2 =a t1.
+Proof.
+  induction 1.
+  - apply aeq_refl.
+  - apply aeq_abs_same; assumption.
+  - apply aeq_abs_diff.
+    -- apply aux_not_equal; assumption.
+    -- apply fv_nom_swap with x y t2 in H0.
+       apply aeq_fv_nom in H1.
+       rewrite H1; assumption.
+    -- apply aeq_swap2 with x y.
+       rewrite swap_involutive.
+       rewrite swap_symmetric.
+       assumption.
+  - apply aeq_app; assumption.
+  - apply aeq_sub_same; assumption.
+  - apply aeq_sub_diff.
+    -- assumption.
+    -- apply aux_not_equal. assumption.
+    -- apply aeq_fv_nom in H2. rewrite H2.
+       apply fv_nom_swap. assumption.
+    -- rewrite swap_symmetric. apply aeq_swap2 with y x.
+       rewrite swap_involutive. assumption.
+Qed.
+(* end hide *)
+
+(** The key point of the nominal approach is that the swap operation is stable under $\alpha$-equivalence in the sense that, $t_1 =_\alpha t_2$ if, and only if $\swap{x}{y}{t_1} =_\alpha \swap{x}{y}{t_2}$. Note that this is not true for renaming substitutions: in fact, $\lambda_x.z =_\alpha \lambda_y.z$, but $(\lambda_x.z)\msub{z}{x} = \lambda_x.x \neq_\alpha \lambda_y.x (\lambda_y.z)\msub{z}{x}$, assuming that $x \neq y$. This stability result is formalized as follows: *)
+
 Corollary aeq_swap: forall t1 t2 x y, t1 =a t2 <-> (swap x y t1) =a (swap x y t2).
 Proof.
   intros. split.
@@ -1463,6 +1093,7 @@ Proof.
   - apply aeq_swap2.
 Qed.
 
+(* begin hide *)
 Lemma aeq_abs: forall t x y, y `notin` fv_nom t -> (n_abs y (swap x y t)) =a (n_abs x t).
 Proof.
   intros. case (x == y); intros; subst.
@@ -1590,6 +1221,54 @@ Proof.
                **** apply swap_symmetric.
 Qed.
 
+Lemma aeq_same_abs: forall x t1 t2, n_abs x t1 =a n_abs x t2 -> t1 =a t2.
+Proof.
+  intros. inversion H.
+  - assumption.
+  - rewrite swap_id in H6; assumption.
+Qed.
+
+Lemma aeq_diff_abs: forall x y t1 t2, (n_abs x t1) =a (n_abs y t2) -> t1 =a (swap x y t2).
+Proof.
+  intros. inversion H; subst.
+  - rewrite swap_id; assumption.
+  - rewrite swap_symmetric; assumption.
+Qed.
+
+Lemma aeq_same_sub: forall x t1 t1' t2 t2', (n_sub t1 x t2) =a (n_sub t1' x t2') -> t1 =a t1' /\ t2 =a t2'.
+Proof.
+  intros. inversion H; subst.
+  - split; assumption.
+  - split.
+    + rewrite swap_id in H9; assumption.
+    + assumption.
+Qed.
+
+Lemma aeq_diff_sub: forall x y t1 t1' t2 t2', (n_sub t1 x t2) =a (n_sub t1' y t2') -> t1 =a (swap x y t1') /\ t2 =a t2'.
+Proof.
+  intros. inversion H; subst.
+  - split.
+    + rewrite swap_id; assumption.
+    + assumption.
+  - split.
+    + rewrite swap_symmetric; assumption.
+    + assumption.
+Qed.
+
+Lemma aeq_sub: forall t1 t2 x y, y `notin` fv_nom t1 -> (n_sub (swap x y t1) y t2) =a (n_sub t1 x t2).
+Proof.
+  intros. case (x == y); intros; subst.
+  - rewrite swap_id; apply aeq_refl.
+  - apply aeq_sub_diff.
+    -- apply aeq_refl.
+    -- apply aux_not_equal; assumption.
+    -- assumption.
+    -- apply aeq_refl.
+Qed.
+(* end hide *)
+
+(** There are several interesting auxiliary properties that need to be proved before achieving the substitution lemma. In what follows, we refer only to the tricky or challenging ones, but the interested reader can have a detailed look in the source files. Note that, swaps are introduced in proofs by the rules $\mbox{\it aeq}\_\mbox{\it abs}\_\mbox{\it diff}$ and $\mbox{\it aeq}\_\mbox{\it sub}\_\mbox{\it diff}$. As we will see, the proof steps involving these rules are trick because a naïve strategy can easily result in a proofless branch. so that one can establish the $\alpha$-equivalence between two abstractions or two explicit substitutions with different binders. The following proposition states when two swaps with a common name collapse, and it is used in the transitivity proof of [aeq]: *)
+
 Lemma aeq_swap_swap: forall t x y z, z `notin` fv_nom t -> x `notin` fv_nom t -> (swap z x (swap x y t)) =a (swap z y t).
 Proof.
   intros. case (x == z); intros; subst.
@@ -1606,31 +1285,133 @@ Proof.
            + assumption.
 Qed.
 
-Lemma aeq_sym: forall t1 t2, t1 =a t2 -> t2 =a t1.
+(** * The metasubstitution operation of the $\lambda$-calculus *)
+
+(** The main operation of the $\lambda$-calculus is the $\beta$-reduction that express how to evaluate a function applied to a given argument: $(\lambda_x.t)\ u \to_{\beta} \metasub{t}{x}{u}$. In a less formal context, the concept of $\beta$-reduction means that the result of evaluating the function $(\lambda_x.t)$ with argument $u$ is obtained by substituting $u$ for the free ocurrences of the variable $x$ in $t$. Moreover, it is a capture free substitution in the sense that no free variable becomes bound after the substitution. This operation is in the meta level because it is outside the grammar of the $\lambda$-calculus, and that's why it is called metasubstitution. As a metaoperation, its definition usually comes with a degree of informality. For instance, Barendregt%\cite{barendregtLambdaCalculusIts1984}% defines it as follows: %\vspace{.5cm}%
+$\metasub{t}{x}{u} = \left\{
+ \begin{array}{ll}
+  u, & \mbox{ if } t = x; \\
+  y, & \mbox{ if } t = y \mbox{ and } x \neq y; \\
+  \metasub{t_1}{x}{u}\ \metasub{t_2}{x}{u}, & \mbox{ if } t = \metasub{(t_1\ t_2)}{x}{u}; \\
+  \lambda_y.(\metasub{t_1}{x}{u}), & \mbox{ if } t = \lambda_y.t_1.
+ \end{array}\right.$ %\vspace{.5cm}%
+%\noindent% where it is assumed the so called "Barendregt's variable convention": if $t_1, t_2, \ldots, t_n$ occur in a certain mathematical context (e.g. definition, proof), then in these terms all bound variables are chosen to be different from the free variables. This means that we are assumming that both $x \neq y$ and $y\notin fv(u)$ in the case $t = \lambda_y.t_1$. This approach is very convenient in informal proofs because it avoids having to rename bound variables. In order to formalize the capture free substitution of the $\lambda$-calculus, %{\it i.e.}% the metasubstitution, a renaming is performed whenever it is propagated inside a binder. In our case, there are two binders: the abstraction and the explicit substitution. 
+
+Let $t$ and $u$ be terms, and $x$ a variable. The result of substituting $u$ for the free ocurrences of $x$ in $t$, written $t\msub{x}{u}$ is defined as follows:%\newline%
+%\begin{equation}\label{msubst}
+\metasub{t}{x}{u} = \left\{
+ \begin{array}{ll}
+  u, & \mbox{ if } t = x; \\
+  y, & \mbox{ if } t = y \mbox{ and } x \neq y; \\
+  \metasub{t_1}{x}{u}\ \metasub{t_2}{x}{u}, & \mbox{ if } t = \metasub{(t_1\ t_2)}{x}{u}; \\
+  \lambda_x.t_1, & \mbox{ if } t = \lambda_x.t_1; \\
+  \lambda_z.(\metasub{(\swap{y}{z}{t_1})}{x}{u}), & \mbox{ if } t = \lambda_y.t_1, x \neq y \mbox{ and } z\notin fv(\lambda_y.t_1)\cup fv(u) \cup \{x\}; \\
+  \esub{t_1}{x}{\metasub{t_2}{x}{u}}, & \mbox{ if } t = \esub{t_1}{x}{t_2}; \\
+  \esub{\metasub{(\swap{y}{z}{t_1})}{x}{u}}{z}{\metasub{t_2}{x}{u}}, & \mbox{ if } t = \esub{t_1}{y}{t_2}, x \neq y \mbox{ and } z\notin fv(\esub{t_1}{y}{t_2})\cup fv(u) \cup \{x\}.
+ \end{array}\right.
+\end{equation}%
+
+Note that this function is not structurally recursive due to the swaps in the recursive calls. A structurally recursive version of the function [subst_rec_fun] can be found in the file [nominal.v] of the [Metalib] library%\footnote{\url{https://github.com/plclub/metalib}}%, but it uses the size of the term in which the substitution will be performed as an extra argument that decreases with each recursive call. We write [[x:=u]t] instead of [subst_rec_fun t u x] in the Coq code to represent $\metasub{t}{x}{u}$. The corresponding Coq code is as follows: *)
+
+(* begin hide *)
+Require Import Recdef.
+(* end hide *)
+Function subst_rec_fun (t:n_sexp) (u :n_sexp) (x:atom) {measure size t} : n_sexp :=
+  match t with
+  | n_var y => if (x == y) then u else t
+  | n_abs y t1 => if (x == y) then t else let (z,_) :=
+    atom_fresh (fv_nom u `union` fv_nom t `union` {{x}}) in n_abs z (subst_rec_fun (swap y z t1) u x)
+  | n_app t1 t2 => n_app (subst_rec_fun t1 u x) (subst_rec_fun t2 u x)
+  | n_sub t1 y t2 => if (x == y) then n_sub t1 y (subst_rec_fun t2 u x) else let (z,_) :=
+    atom_fresh (fv_nom u `union` fv_nom t `union` {{x}}) in
+    n_sub (subst_rec_fun (swap y z t1) u x) z (subst_rec_fun t2 u x) 
+end.
 Proof.
-  induction 1.
-  - apply aeq_refl.
-  - apply aeq_abs_same; assumption.
-  - apply aeq_abs_diff.
-    -- apply aux_not_equal; assumption.
-    -- apply fv_nom_swap with x y t2 in H0.
-       apply aeq_fv_nom in H1.
-       rewrite H1; assumption.
-    -- apply aeq_swap2 with x y.
-       rewrite swap_involutive.
-       rewrite swap_symmetric.
-       assumption.
-  - apply aeq_app; assumption.
-  - apply aeq_sub_same; assumption.
-  - apply aeq_sub_diff.
-    -- assumption.
-    -- apply aux_not_equal. assumption.
-    -- apply aeq_fv_nom in H2. rewrite H2.
-       apply fv_nom_swap. assumption.
-    -- rewrite swap_symmetric. apply aeq_swap2 with y x.
-       rewrite swap_involutive. assumption.
+ - intros. simpl. rewrite swap_size_eq. auto.
+ - intros. simpl. lia.
+ - intros. simpl. lia.
+ - intros. simpl. lia.
+ - intros. simpl. lia.
+ - intros. simpl. rewrite swap_size_eq. lia.
+Defined.
+(* begin hide *)
+Definition m_subst (u : n_sexp) (x:atom) (t:n_sexp) :=
+  subst_rec_fun t u x.
+Notation "[ x := u ] t" := (m_subst u x t) (at level 60).
+
+Lemma m_subst_var_eq : forall u x,
+    [x := u](n_var x) = u.
+Proof.
+  intros u x. unfold m_subst. rewrite subst_rec_fun_equation. rewrite eq_dec_refl. reflexivity.
 Qed.
 
+Lemma m_subst_var_neq : forall u x y, x <> y ->
+    [y := u](n_var x) = n_var x.
+Proof.
+  intros u x y H. unfold m_subst. rewrite subst_rec_fun_equation. destruct (y == x) eqn:Hxy.
+  - subst. contradiction.
+  - reflexivity.
+Qed.
+
+Lemma m_subst_app: forall t1 t2 u x, [x := u](n_app t1 t2) = n_app ([x := u]t1) ([x := u]t2).
+Proof.
+  intros t1 t2 u x. unfold m_subst. rewrite subst_rec_fun_equation. reflexivity.
+Qed.
+(* end hide *)
+
+(** The standard proof strategy for the non trivial properties is induction on the structure of the terms. Nevertheless, the builtin induction principle automatically generated for the inductive definition [n_sexp] is not strong enough due to swappings. In fact, in general, the induction hypothesis in the abstraction case, for instance, refer to the body of the abstraction, while the goal involves a swap acting on the body of the abstraction. In order to circunvet this problem, we use an induction principle based on the size of terms: *)
+
+Lemma n_sexp_induction:
+ forall P : n_sexp -> Prop,
+ (forall x, P (n_var x)) ->
+ (forall t1 z, (forall t2 x y, size t2 = size t1 -> P (swap x y t2)) -> P (n_abs z t1)) ->
+ (forall t1 t2, P t1 -> P t2 -> P (n_app t1 t2)) ->
+ (forall t1 t3 z, P t3 -> (forall t2 x y, size t2 = size t1 -> P (swap x y t2)) -> P (n_sub t1 z t3)) -> 
+ (forall t, P t).
+Proof.
+  intros P Hvar Habs Happ Hsub t.
+  remember (size t) as n.
+  generalize dependent t.
+  induction n using strong_induction.
+  intro t; case t.
+  - intros x Hsize.
+    apply Hvar.
+  - intros x t' Hsize.
+    apply Habs.
+    intros t'' x1 x2 Hsize'.
+    apply H with (size t'').
+    + rewrite Hsize'.
+      rewrite Hsize.
+      simpl.
+      apply Nat.lt_succ_diag_r.
+    + symmetry.
+      apply swap_size_eq.
+  - intros. apply Happ.
+    + apply H with ((size t1)).
+      ++ simpl in Heqn. rewrite Heqn.
+         apply le_lt_n_Sm.
+         apply le_plus_l.
+      ++ reflexivity.
+    + apply H with ((size t2)).
+      ++ simpl in Heqn. rewrite Heqn.
+          apply le_lt_n_Sm.
+         apply le_plus_r.
+      ++ reflexivity.
+  - intros. apply Hsub.
+    + apply H with ((size t2)).
+      ++ simpl in Heqn. rewrite Heqn.
+          apply le_lt_n_Sm.
+         apply le_plus_r.
+      ++ reflexivity.
+    + intros. apply H with ((size (swap x0 y t0))).
+      ++ rewrite swap_size_eq. rewrite H0.
+         simpl in Heqn. rewrite Heqn.
+         apply le_lt_n_Sm.
+         apply le_plus_l.
+      ++ reflexivity.
+Qed. 
+
+(* begin hide *)
 Lemma aeq_trans: forall t1 t2 t3, t1 =a t2 -> t2 =a t3 -> t1 =a t3.
 Proof.
   induction t1 using n_sexp_induction.
@@ -1877,111 +1658,7 @@ Proof.
                          assumption.
                     * assumption.
                     * assumption.
-Qed.                 
-
-
-(*
-Lemma swap_comp : forall x y z t, x `notin` fv_nom t -> y `notin` fv_nom t ->
-    (swap x y (swap y z t)) =a (swap x z t).
-Proof.
-  induction t.
-  - intros H1 H2. simpl. destruct (x0 == z). 
-    + subst. destruct (x == z). 
-      * subst. destruct (y == z).
-        ** subst. unfold swap_var. rewrite eq_dec_refl. rewrite eq_dec_refl. apply aeq_refl.
-        ** unfold swap_var. rewrite eq_dec_refl. destruct (z == y).
-            *** rewrite eq_dec_refl. subst. apply aeq_refl.
-            *** destruct (y == z). 
-                **** contradiction.
-                **** rewrite eq_dec_refl. apply aeq_refl.
-      * unfold swap_var. destruct (z == y).
-        ** destruct (z == x). 
-            *** subst. contradiction.
-            *** subst. rewrite eq_dec_refl. apply aeq_refl.
-        ** rewrite eq_dec_refl. 
-            *** destruct (y == x).
-                **** subst. destruct (z == x).
-                      ***** contradiction.
-                      ***** apply aeq_refl.
-                **** rewrite eq_dec_refl. destruct (z == x).
-                      ***** subst. apply aeq_refl.
-                      ***** apply aeq_refl.
-    + unfold swap_var. destruct (x0 == y).
-      * subst. destruct (z == x). 
-        ** subst. destruct (y == x). 
-            *** subst. contradiction.
-            *** apply aeq_refl.
-        ** destruct (z == y).
-            *** subst. destruct (y == x). 
-                **** contradiction.
-                **** rewrite eq_dec_refl. apply aeq_refl.
-            *** destruct (y == x). 
-                **** apply aeq_refl.
-                **** destruct (y == z).
-                      ***** subst. contradiction.
-                      ***** simpl in H2. apply notin_singleton_is_false in H2. exfalso. assumption.
-      * destruct (x0 == z). 
-        ** subst. destruct (y == x). 
-            *** subst. contradiction.
-            *** rewrite eq_dec_refl. destruct (z == x).
-                **** subst. contradiction.
-                **** contradiction.
-        ** destruct (x0 == x).
-            *** subst. apply notin_singleton_is_false in H1. exfalso. assumption.
-            *** subst. destruct (x0 == y). 
-                **** subst. contradiction.
-                **** apply aeq_refl.
-  - intros H1 H2. simpl in *. apply notin_remove_1 in H1.  apply notin_remove_1 in H2. destruct H1.
-    + subst.
-    + Admitted.
-
-    unfold swap_var. destruct (x0 == z). 
-    + destruct (x0 == y). 
-      * subst. destruct (y == x). 
-        ** subst. repeat rewrite swap_id. apply aeq_refl.
-        ** rewrite eq_dec_refl. apply aeq_abs_same. apply IHt.
-          *** admit.
-          *** admit.
-      * subst. destruct (y == x). 
-        ** destruct (z == x).
-          *** subst. repeat rewrite swap_id. apply aeq_refl.
-          *** subst. repeat rewrite swap_id. apply aeq_refl.
-        ** rewrite eq_dec_refl. destruct (z == x).
-          *** subst. apply aeq_abs_same. apply IHt.
-              **** admit.
-              **** admit.
-          *** apply aeq_abs_same. apply IHt.
-              **** admit.
-              **** admit.
-    + destruct (x0 == y). 
-      * subst. destruct (y == x). 
-        ** subst. destruct (z == x).
-          *** subst. contradiction.
-          *** rewrite swap_id. apply aeq_refl.
-        ** destruct (z == x). 
-          *** subst. apply aeq_abs_same. apply IHt.
-              **** admit.
-              **** admit.
-          *** destruct (z == y). 
-              **** subst. contradiction.
-              **** admit.
-      * destruct (x0 == x).
-        ** subst. admit.
-        ** destruct (x0 == y).
-          *** subst. contradiction.
-          *** apply aeq_abs_same. apply IHt.
-              **** admit.
-              **** admit.
-   - intros H1 H2. simpl. apply aeq_app.
-    + apply IHt1. 
-      * simpl in H1. apply notin_union_1 in H1. assumption.
-      * simpl in H2. apply notin_union_1 in H2. assumption.
-    + apply IHt2. 
-      * simpl in H1. apply notin_union_2 in H1. assumption.
-      * simpl in H2. apply notin_union_2 in H2. assumption.
-  - intros H1 H2. simpl. admit.
-
-Admitted. *)
+Qed.
 
 Require Import Setoid Morphisms.
 
@@ -1992,344 +1669,9 @@ Proof.
   - unfold Symmetric. apply aeq_sym.
   - unfold Transitive. apply aeq_trans.
 Qed.
+(* end hide *)
 
-Lemma aeq_same_abs: forall x t1 t2, n_abs x t1 =a n_abs x t2 -> t1 =a t2.
-Proof.
-  intros. inversion H.
-  - assumption.
-  - rewrite swap_id in H6; assumption.
-Qed.
-
-Lemma aeq_diff_abs: forall x y t1 t2, (n_abs x t1) =a (n_abs y t2) -> t1 =a (swap x y t2).
-Proof.
-  intros. inversion H; subst.
-  - rewrite swap_id; assumption.
-  - rewrite swap_symmetric; assumption.
-Qed.
-
-Lemma aeq_same_sub: forall x t1 t1' t2 t2', (n_sub t1 x t2) =a (n_sub t1' x t2') -> t1 =a t1' /\ t2 =a t2'.
-Proof.
-  intros. inversion H; subst.
-  - split; assumption.
-  - split.
-    + rewrite swap_id in H9; assumption.
-    + assumption.
-Qed.
-
-Lemma aeq_diff_sub: forall x y t1 t1' t2 t2', (n_sub t1 x t2) =a (n_sub t1' y t2') -> t1 =a (swap x y t1') /\ t2 =a t2'.
-Proof.
-  intros. inversion H; subst.
-  - split.
-    + rewrite swap_id; assumption.
-    + assumption.
-  - split.
-    + rewrite swap_symmetric; assumption.
-    + assumption.
-Qed.
-
-Lemma aeq_sub: forall t1 t2 x y, y `notin` fv_nom t1 -> (n_sub (swap x y t1) y t2) =a (n_sub t1 x t2).
-Proof.
-  intros. case (x == y); intros; subst.
-  - rewrite swap_id; apply aeq_refl.
-  - apply aeq_sub_diff.
-    -- apply aeq_refl.
-    -- apply aux_not_equal; assumption.
-    -- assumption.
-    -- apply aeq_refl.
-Qed.
-               
-(*
-Lemma swap_comp: forall t x y z,
-    x <> z -> y <> z -> x `notin` fv_nom t -> y `notin` fv_nom t -> aeq (swap y x (swap y z t)) (swap x z t).
-Proof.
-Admitted.
-
-false: take t = y or t = x
-Lemma swap_trans: forall t x y z, (swap x y (swap y z t)) = swap x z t.
-Proof.
-  induction t.
-  - intros. simpl. unfold swap_var. default_simp.
-    + apply notin_singleton_is_false in H.
-      contradiction.
-    + apply notin_singleton_is_false in H0.
-      contradiction.
-  - intros. simpl. unfold swap_var.
-    case (x == y).
-    + intro H'; subst.
-      case (z == x0).
-      * intro H'; subst.
-        case (y == x0).
-        ** intro H'; subst.
-           rewrite swap_involutive.
-           rewrite swap_id.
-           reflexivity.
-        ** intro H'.
-           rewrite IHt.
-           *** reflexivity.
-           *** simpl in H.
-               apply notin_remove_1 in H.
-               destruct H.
-               **** contradiction.
-               **** assumption.
-           *** simpl in H0.
-               apply notin_remove_1 in H0.
-               destruct H0.
-               **** contradiction.
-               **** assumption.
-      * intro H; case (z == y).
-        ** intro H'; subst.
-           case (y == x0).
-           *** intro H'; contradiction.
-           *** intro H'; case (y == y).
-               **** intro H''; reflexivity.
-               **** intro H''; contradiction.
-        ** intro H'; case (y == x0).
-           *** intro H''; subst.
-               reflexivity.
-           *** intro H''; case (y == z).
-               **** intro H'''; subst.
-                    contradiction.
-               **** Admitted.
-
-  - intros. simpl. unfold swap_var. default_simp.
-  - intros. simpl. unfold swap_var. default_simp. 
-
-Lemma aeq_diff_abs': forall x y t1 t2, x `notin` fv_nom t2 -> t1 =a (swap x y t2) -> (n_abs x t1) =a (n_abs y t2).
-Proof.
-  intros x y t1 t2 Hnotin H.
-  inversion H; subst.
-  - rewrite H2.
-    rewrite swap_symmetric.
-    apply aeq_abs; assumption.
-  - inversion H. rewrite swap_symmetric; assumption.
-Qed.
-
-Lemma aeq_abs_diff_swap: forall t1 t2 x y z, x <> y -> z `notin` fv_nom t1 -> z `notin` fv_nom t2 -> aeq (n_abs x t1) (n_abs y t2) -> aeq (swap x z t1) (swap y z t2).
-Proof.
-  intros t1 t2 x y z Hneq Hnotin1 Hnotin2 Haeq.
-  induction Haeq.
-  -
-  Admitted.
- *)
-    
-
-(** ** Capture-avoiding substitution *)
-
-(** We need to use size to define capture avoiding
-    substitution. Because we sometimes swap the name of the
-    bound variable, this function is _not_ structurally
-    recursive. So, we add an extra argument to the function
-    that decreases with each recursive call. 
-
-Fixpoint subst_rec (n:nat) (t:n_sexp) (u :n_sexp) (x:atom)  : n_sexp :=
-  match n with
-  | 0 => t
-  | S m => match t with
-          | n_var y =>
-            if (x == y) then u else t
-          | n_abs y t1 =>
-            if (x == y) then t
-            else
-              (* rename to avoid capture *)
-              let (z,_) :=
-                  atom_fresh (fv_nom u `union` fv_nom t `union` {{x}}) in
-                 n_abs z (subst_rec m (swap y z t1) u x)
-          | n_app t1 t2 =>
-            n_app (subst_rec m t1 u x) (subst_rec m t2 u x)
-          | n_sub t1 y t2 =>
-            if (x == y) then n_sub t1 y (subst_rec m t2 u x)
-            else
-              (* rename to avoid capture *)
-              let (z,_) :=
-                  atom_fresh (fv_nom u `union` fv_nom t `union` {{x}}) in
-                 n_sub  (subst_rec m (swap y z t1) u x) z (subst_rec m t2 u x) 
-           end
-  end. *)
-
-Require Import Recdef.
-
-Function subst_rec_fun (t:n_sexp) (u :n_sexp) (x:atom) {measure size t} : n_sexp :=
-  match t with
-  | n_var y =>
-      if (x == y) then u else t
-  | n_abs y t1 =>
-      if (x == y) then t
-      else let (z,_) :=
-                  atom_fresh (fv_nom u `union` fv_nom t `union` {{x}}) in
-                n_abs z (subst_rec_fun (swap y z t1) u x)
-  | n_app t1 t2 =>
-      n_app (subst_rec_fun t1 u x) (subst_rec_fun t2 u x)
-  | n_sub t1 y t2 =>
-      if (x == y) then n_sub t1 y (subst_rec_fun t2 u x)
-      else let (z,_) :=
-                  atom_fresh (fv_nom u `union` fv_nom t `union` {{x}}) in
-              n_sub  (subst_rec_fun (swap y z t1) u x) z (subst_rec_fun t2 u x) 
-           end.
-Proof.
- - intros. simpl. rewrite swap_size_eq. auto.
- - intros. simpl. lia.
- - intros. simpl. lia.
- - intros. simpl. lia.
- - intros. simpl. lia.
- - intros. simpl. rewrite swap_size_eq. lia.
-Defined.
-
-(*
-Inductive meta_subst: n_sexp -> atom -> n_sexp -> n_sexp -> Prop :=
-| meta_var_eq: forall x u, meta_subst (n_var x) x u u
-| meta_var_neq: forall x y u, x <> y -> meta_subst (n_var y) x u (n_var y)
-| meta_app: forall t1 t1' t2 t2' x u, meta_subst t1 x u t1' -> meta_subst t2 x u t2' -> meta_subst (n_app t1 t2) x u (n_app t1' t2')
-| meta_abs_eq: forall t x u, meta_subst (n_abs x t) x u (n_abs x t) 
-| meta_abs_neq1: forall t x y u v, y `notin` fv_nom u -> meta_subst t x u v -> meta_subst (n_abs y t) x u v 
-| meta_abs_neq2: forall t x y z u v, y `in` fv_nom u -> z `notin` (fv_nom t `union` fv_nom u `union` {{x}} `union` {{y}}) -> meta_subst (swap y z t) x u v -> meta_subst (n_abs y t) x u v
-| meta_sub_eq: forall t1 t2 t2' x u, meta_subst t2 x u t2' -> meta_subst (n_sub t1 x t2) x u (n_sub t1 x t2') 
-| meta_sub_neq1: forall t1 t1' t2 t2' x y u, x <> y ->  y `notin` fv_nom u ->  meta_subst t1 x u t1' -> meta_subst t2 x u t2' -> meta_subst (n_sub t1 y t2) x u (n_sub t1' x t2')
-| meta_sub_neq2: forall t1 t1' t2 t2' x y z u, x <> y ->  y `in` fv_nom u -> z `notin` (fv_nom t1 `union` fv_nom u `union` {{x}} `union` {{y}}) ->  meta_subst (swap y z t1) x u t1' -> meta_subst t2 x u t2' -> meta_subst (n_sub t1 y t2) x u (n_sub t1' x t2'). 
-
-Lemma fv_nom_remove: forall t u v x y, y `notin` fv_nom u -> y `notin` remove x (fv_nom t) -> meta_subst t x u v ->  y `notin` fv_nom v.
-Proof. 
-  intros t u v x y H1 H2 H3. induction H3.
-  - assumption.
-  - apply notin_remove_1 in H2. destruct H2.
-    + subst. apply notin_singleton. apply aux_not_equal; assumption.
-    + assumption.
-  - simpl in *. rewrite remove_union_distrib in H2. assert (H3 := H2). apply notin_union_1 in H2. apply notin_union_2 in H3. apply notin_union.
-    + apply IHmeta_subst1; assumption.
-    + apply IHmeta_subst2; assumption.
-  - simpl in *. rewrite double_remove in H2. assumption.
-  - apply IHmeta_subst.
-    + assumption.
-    + simpl in H2.
-
-      rewrite remove_symmetric in H2. apply notin_remove_1 in H2. destruct H2.
-      * subst. assumption.
-      *)
-        
-(** The definitions subst_rec and subst_rec_fun are alpha-equivalent. 
-Theorem subst_rec_fun_equiv: forall t u x, (subst_rec (size t) t u x) =a (subst_rec_fun t u x).
-Proof.
-  intros t u x. functional induction (subst_rec_fun t u x).
-  - simpl. rewrite e0. apply aeq_refl.
-  - simpl. rewrite e0. apply aeq_refl.
-  - simpl. rewrite e0. apply aeq_refl.
-  - simpl. rewrite e0. destruct (atom_fresh (Metatheory.union (fv_nom u) (Metatheory.union (remove y (fv_nom t1)) (singleton x)))).  admit.
-  - simpl. admit.
-  - simpl. rewrite e0. admit.
-  - simpl. rewrite e0.
-Admitted.
-
-Require Import EquivDec.
-Generalizable Variable A.
-
-Definition equiv_decb `{EqDec A} (x y : A) : bool :=
-  if x == y then true else false.
-
-Definition nequiv_decb `{EqDec A} (x y : A) : bool :=
-  negb (equiv_decb x y).
-
-Infix "==b" := equiv_decb (no associativity, at level 70).
-Infix "<>b" := nequiv_decb (no associativity, at level 70).
-
-Parameter Inb : atom -> atoms -> bool.
-Definition equalb s s' := forall a, Inb
-
-Function subst_rec_b (t:n_sexp) (u :n_sexp) (x:atom) {measure size t} : n_sexp :=
-  match t with
-  | n_var y =>
-      if (x == y) then u else t
-  | n_abs y t1 =>
-      if (x == y) then t
-      else if (Inb y (fv_nom u)) then let (z,_) :=
-                  atom_fresh (fv_nom u `union` fv_nom t `union` {{x}}) in
-                                      n_abs z (subst_rec_b (swap y z t1) u x)
-                                            else n_abs y (subst_rec_b t1 u x)
-  | n_app t1 t2 =>
-      n_app (subst_rec_b t1 u x) (subst_rec_b t2 u x)
-  | n_sub t1 y t2 =>
-      if (x == y) then n_sub t1 y (subst_rec_b t2 u x)
-      else if (Inb y (fv_nom u)) then let (z,_) :=
-                  atom_fresh (fv_nom u `union` fv_nom t `union` {{x}}) in
-                                      n_sub  (subst_rec_b (swap y z t1) u x) z (subst_rec_b t2 u x)
-                                             else n_sub (subst_rec_b t1 u x) y (subst_rec_b t2 u x)
-           end.
-Proof.
- - intros. simpl. rewrite swap_size_eq. auto.
- - intros. simpl. lia.
- - intros. simpl. lia.
- - intros. simpl. lia.
- - intros. simpl. lia.
- - intros. simpl. rewrite swap_size_eq. lia.
-Defined. *)
-
-(** Our real substitution function uses the size of the size of the term
-    as that extra argument. *)
-
-Definition m_subst (u : n_sexp) (x:atom) (t:n_sexp) :=
-  subst_rec_fun t u x.
-Notation "[ x := u ] t" := (m_subst u x t) (at level 60).
-
-(** The lemmas following say that the application of the meta-substitution to the same variable that is in it return the expression in the meta-substitution. The next lemma says that if the variables in the meta-substitution and in the expression are different, that is equal to the variable expression. **)
-
-Lemma m_subst_var_eq : forall u x,
-    [x := u](n_var x) = u.
-Proof.
-  intros u x. unfold m_subst. rewrite subst_rec_fun_equation. rewrite eq_dec_refl. reflexivity.
-Qed.
-
-Lemma m_subst_var_neq : forall u x y, x <> y ->
-    [y := u](n_var x) = n_var x.
-Proof.
-  intros u x y H. unfold m_subst. rewrite subst_rec_fun_equation. destruct (y == x) eqn:Hxy.
-  - subst. contradiction.
-  - reflexivity.
-Qed.
-
-(** The behaviour of free variables in a metasubstitution. *)
-(* probably not needed now
-Lemma fv_nom_m_subst_in: forall t u x, x `in` fv_nom t -> fv_nom ([x := u] t) [=] (union (remove x (fv_nom t)) (fv_nom u)).
-Proof.
-  intros t u x. unfold m_subst. functional induction (subst_rec_fun t u x).
-  - intros H. rewrite remove_singleton_empty. rewrite AtomSetProperties.empty_union_1.
-    + reflexivity.
-    + unfold AtomSetImpl.Empty. auto.
-  - intro H. simpl in H. apply singleton_iff in H. symmetry in H. contradiction.
-  - intro H. simpl in H. pose proof notin_remove_3'. specialize (H0 x x (fv_nom t1)). assert (H': x = x). { reflexivity. } apply H0 in H'. contradiction.
-  - simpl. intro H. rewrite IHn. Admitted. 
-
-Lemma remove_fv_nom_swap: forall t x y, x `notin` fv_nom t -> remove x (fv_nom (swap y x t)) [=] remove y (fv_nom t).
-Proof.
-  induction t using n_sexp_induction.
-  - intros x' y Hfv. simpl in *. apply notin_singleton_1 in Hfv. unfold swap_var. destruct (x == y).
-    + subst. repeat rewrite remove_singleton_empty. reflexivity.
-    + destruct (x == x').
-      * contradiction.
-      * rewrite AtomSetProperties.remove_equal.
-        ** symmetry. rewrite AtomSetProperties.remove_equal.
-           *** reflexivity.
-           *** apply notin_singleton. assumption.
-        ** apply notin_singleton. assumption.
-  - intros x y Hfv. simpl in *. pose proof Hfv as Hfv'. apply notin_remove_1 in Hfv. destruct Hfv.
-    + subst. case (x == y).
-      * intro Heq. subst. rewrite swap_id. rewrite swap_var_id. reflexivity.
-      * intro Hneq. unfold swap_var. destruct (x == y).
-        ** contradiction.
-        ** rewrite eq_dec_refl. symmetry. rewrite remove_symmetric. symmetry. apply swap_remove_reduction.
-    + case (x == y).
-      * intro Heq. subst. rewrite swap_var_id. rewrite swap_id. reflexivity.
-      * intro Hneq. unfold swap_var. destruct (z == y).
-        ** subst. repeat rewrite double_remove. specialize (H t x x). rewrite swap_id in H. assert (Ht: size t = size t). { reflexivity. } apply H.
-           *** reflexivity.
-           *** assumption.
-        ** destruct (z == x).
-           *** subst. symmetry. rewrite remove_symmetric. symmetry. apply swap_remove_reduction.
-           *** rewrite remove_symmetric. symmetry. rewrite remove_symmetric. symmetry. specialize (H t x x). rewrite swap_id in H. assert (Ht: size t = size t). { reflexivity. } rewrite H.
-               **** reflexivity.
-               **** reflexivity.
-               **** assumption.
-  - Admitted. *)
-
-(** The following lemma defines that if the variable in the meta-substitution is not in the free variables in the expression the meta-substitution is applied to, then the meta-substitution is alpha-equivalent to the expression itself. **)
-(** The proof of this lemma is done using the induction in the expression the meta-substitution is applied to and the definition of the meta-substittution was also used in all cases. The application and the variable cases are done similarly. For both the abstraction and explicit substitution, it was necessary to compare the variables of the meta-substitition and the expression. The lemmas for alpha-substitution equalities above were used in the proofs for abstraction and explicit substitution.**)
+(** The following lemma states that if $x \notin fv(t)$ then $\metasub{t}{x}{u} =_\alpha t$. In informal proofs the conclusion of this lemma is usually stated as a syntactic equality, %{\i.e.}% $\metasub{t}{x}{u} = t$ instead of the $\alpha$-equivalence, but due to the changes of the names of the bound variables when the metasubstitution is propagated inside an abstraction or inside an explicit substitution, syntactic equality does not hold here. *)
 
 Lemma m_subst_notin: forall t u x, x `notin` fv_nom t -> [x := u]t =a t.
 Proof.
@@ -2365,7 +1707,7 @@ Proof.
       * apply aeq_refl.
       * apply notin_union_2 in Hfv. apply IHt1. assumption.
     + case (x0 == z).
-      * intro Heq. subst.  apply aeq_sub_same.
+      * intro Heq. subst. apply aeq_sub_same.
         ** apply aeq_trans with (swap z z t1). apply H.
            *** reflexivity.
            *** rewrite swap_id. apply notin_union_1 in Hfv. apply notin_remove_1 in Hfv. destruct Hfv.
@@ -2381,53 +1723,22 @@ Proof.
            *** assumption.
         ** apply H.
            *** reflexivity.
-           *** apply fv_nom_remove_swap.
-               **** repeat apply notin_union_2 in n. apply notin_singleton_1 in n. assumption.
-               **** assumption.
-               **** apply notin_union_1 in Hfv. apply notin_remove_1 in Hfv. destruct Hfv.
-                    ***** symmetry in H0. contradiction.
-                    ***** assumption.
+           *** apply notin_union_1 in Hfv. apply notin_remove_1 in Hfv. destruct Hfv. 
+               **** symmetry in H0. contradiction. 
+               **** repeat apply notin_union_2 in n. apply notin_singleton_1 in n. apply fv_nom_remove_swap; assumption.
 Qed.
+(** %\noindent{\bf Proof.}% The proof is done by induction on the size of the term [t] using the [n_sexp_induction] principle. One interesting case is when $t = \lambda_y.t_1$ and $x \neq y$. In this case, we have to prove that $(\lambda_y.t_1)\msub{x}{u} =_\alpha \lambda_y.t_1$. The induction hypothesis express the fact that every term with the same size as the body of the abstraction $t_1$ satisfies the property to be proven:
 
-(** I was necessary to use an axiom stating that if two atoms are equal, they have the same elements in the following proof. **)
+$\forall t'\ x\ y, |t'| = |t_1| \to \forall u\ x', x' \notin fv(\swap{x}{y}{t'}) \to (\swap{x}{y}{t'})\msub{x'}{u} =_\alpha \swap{x}{y}{t'}$.
 
-Axiom Eq_implies_equality: forall s s': atoms, s [=] s' -> s = s'.
+Therefore, according to the function [subst_rec_fun], the variable $y$ will be renamed to a new name, say $z$, such that $z \notin fv(\lambda_y.t_1) \cup fv(u) \cup \{x\}$, and we have to prove that $\lambda_z.(\swap{z}{y}{t_1})\msub{x}{u} =_\alpha \lambda_y.t_1$. Since $z \notin fv(\lambda_y.t_1) = fv(t_1)\backslash \{y\}$, there are two cases:
+ %\begin{enumerate}
+   \item $z = y$: In this case, we have to prove that $\lambda_z.(\swap{z}{z}{t_1})\msub{x}{u} =_\alpha \lambda_z.t_1$. By the rule $\mbox{\it aeq}\_\mbox{\it abs}\_\mbox{\it same}$ we get $(\swap{z}{z}{t_1})\msub{x}{u} =_\alpha t_1$, but in order to apply the induction hypothesis the body of the metasubstitution and the term in the right hand side need to be the same and both need to be a swap. For this reason, we use the transitivity of $\alpha$-equivalence with $\swap{z}{z}{t_1}$ as intermediate term. The first subcase is proved by the induction hypothesis, and the second one is proved by the reflexivity of $\alpha$-equivalence.
+\item $z \neq y$: In this case, $x \notin fv(t)$ and we can apply the rule $\mbox{\it aeq}\_\mbox{\it abs}\_\mbox{\it diff}$. The new goal is $(\swap{z}{y}{t_1})\msub{x}{u} =_\alpha \swap{z}{y}{t_1}$ which holds by the induction hypothesis, since $|\swap{z}{y}{t_1}| = |t_1|$ and $x \notin fv(\swap{z}{y}{t_1})$ because $x \neq z$, $x \neq y$ and $x \notin fv(t)$.
+  \end{enumerate}%
+ The explicit substitution case is also interesting, but it follows a similar strategy used in the abstraction case for $t_1$. For $t_2$ the result follows from the induction hypothesis. $\hfill\Box$ *)
 
-(* probably not needed now
-Lemma fv_nom_m_subst_notin: forall t u x, x `notin` fv_nom t -> fv_nom ([x := u] t) [=] fv_nom t.
-Proof. 
-  induction t using n_sexp_induction.
-  - intros u x' Hfv. simpl in *. rewrite AtomSetProperties.remove_equal. 
-    + unfold m_subst. rewrite subst_rec_fun_equation. destruct (x' == x).
-      * apply notin_singleton_1 in Hfv. symmetry in e. contradiction.
-      * reflexivity.
-    + assumption.
-  - intros u x Hfv. simpl in *. unfold m_subst in *. rewrite subst_rec_fun_equation. 
-    * destruct (x == z). 
-      ** simpl. symmetry. rewrite AtomSetProperties.remove_equal.
-         *** reflexivity.
-         *** assumption.
-      ** destruct (atom_fresh (union (fv_nom u) (union (fv_nom (n_abs z t)) (singleton x)))). case (x0 == z).
-         *** intro Heq. subst. rewrite swap_id. simpl in  *. pose proof m_subst_notin. pose proof Hfv as Hfv'. apply notin_remove_1 in Hfv'. destruct Hfv' as [Hfv'' |Hfv'''].
-             **** symmetry in Hfv''. contradiction.
-             **** apply (H0 _ u) in Hfv'''. unfold m_subst in Hfv'''. apply aeq_fv_nom in Hfv'''. apply Eq_implies_equality in Hfv'''. rewrite Hfv'''. symmetry. apply AtomSetProperties.remove_equal. assumption.
-         *** intro Hneq. simpl in *. rewrite H.
-             **** rewrite remove_symmetric. rewrite remove_fv_nom_swap.
-                  ***** reflexivity.
-                  ***** apply notin_union_2 in n0. apply notin_union_1 in n0. apply notin_remove_1 in n0. destruct n0.
-                  ****** symmetry in H0. contradiction.
-                  ****** assumption.
-             **** reflexivity.
-             **** apply fv_nom_remove_swap.
-                  ***** repeat apply notin_union_2 in n0. apply notin_singleton_1 in n0. assumption.
-                  ***** assumption.
-                  ***** apply notin_remove_1 in Hfv. destruct Hfv.
-                  ****** symmetry in H0. contradiction.
-                  ****** assumption. Admitted. *)
-
-(** The lemma below states that if a variable is not in the free-variables the application of a meta-substitution on an expression, it is not in the of free-variables of the expression the meta-substitution is applied to, removing the variable in the meta-substitution and it is not in the free variables of the expression inside of the meta-substitution. **)
-(** The proof of the lemma is done by functional induction in the meta substitution. The variable and application cases are trivial, and so are the first ones in the abstraction and explicit substitution. The second case in the abstraction is solved by comparing the variables inside the meta-substitution and the abstraction. The same is done for the left side os the explicit substitution, and its right side is solved similarly to the application.**)
-
+(* begin hide *)
 Lemma fv_nom_remove: forall t u x y, y `notin` fv_nom u -> y `notin` remove x (fv_nom t) ->  y `notin` fv_nom ([x := u] t).
 Proof. 
   intros t u x y H0 H1. unfold m_subst. functional induction (subst_rec_fun t u x).
@@ -2507,17 +1818,67 @@ Proof.
         ** assumption.
         ** apply notin_union_2 in H. apply notin_remove_2. assumption.
 Qed.
+(* end hide *)
 
-(** The next lemma states that if the variable in the meta-substitution and the expression the meta- substition is applied to are alpha-equivalent, then the exxpression inside the meta-substition has to be alpha-equivalent in both sides.**)
-(** The proof for this lemma is done on induction in the expression, generating one case for each of the possible expressions and the definition of the meta-substitution is used to complete the proof. **)
+(** We will now prove some stability results for the metasubstitution w.r.t. $\alpha$-equivalence. More precisely, we will prove that if $t =_\alpha t'$ and $u =_\alpha u'$ then $\metasub{t}{x}{u} =_\alpha \metasub{t'}{x}{u'}$, where $x$ is any variable and $t, t', u$ and $u'$ are any [n_sexp] terms. This proof is split in two steps: firstly, we prove that if $u =_\alpha u'$ then $\metasub{t}{x}{u} =_\alpha \metasub{t}{x}{u'}, \forall x, t, u, u'$; secondly, we prove that if $t =_\alpha t'$ then $\metasub{t}{x}{u} =_\alpha \metasub{t'}{x}{u}, \forall x, t, t', u$. These two steps are then combined through the transitivity of the $\alpha$-equivalence relation. Nevertheless, this task were not straighforward. Let's follow the steps of our first trial.*)
+
+Lemma aeq_m_subst_in_trial: forall t u u' x, u =a u' -> ([x := u] t) =a ([x := u'] t).
+Proof.
+  induction t using n_sexp_induction. (** %\noindent{\bf Proof.}% The proof is done by induction on the size of the term [t].*)
+  - intros u u' x' Haeq. unfold m_subst. repeat rewrite subst_rec_fun_equation. destruct (x' == x).
+    + assumption.
+    + apply aeq_refl.
+  - intros u u' x Haeq. unfold m_subst in *. repeat rewrite subst_rec_fun_equation. destruct (x == z). (** The interesting case is when [t] is an abstraction, %{\it i.e.}% $t = \lambda_y.t_1$. We need to prove that $\metasub{(\lambda_y.t_1)}{x}{u} =_\alpha \metasub{(\lambda_y.t_1)}{x}{u'}$.*)      
+    + apply aeq_refl. (** If $x = y$ then the result is trivial.*)
+    + destruct (atom_fresh (union (fv_nom u) (union (fv_nom (n_abs z t)) (singleton x)))). destruct (atom_fresh (union (fv_nom u') (union (fv_nom (n_abs z t)) (singleton x)))). case (x0 == x1). (** Suppose $x \neq y$. The metasubstitution will be propagated inside the abstraction on each side of the $\alpha$-equation, after generating a new name for each side. The new goal is then $\lambda_{x_0}.\metasub{(\swap{y}{x_0}{t_1})}{x}{u} =_\alpha \lambda_{x_1}.\metasub{(\swap{y}{x_1}{t_1})}{x}{u'}$, where $x_0 \notin fv(\lambda_y.t_1) \cup fv(u) \cup \{x\}$ and $x_1 \notin fv(\lambda_y.t_1) \cup fv(u') \cup \{x\}$. The variables $x_0$ and $x_1$ are either the same or different.*)
+      * intro Heq. subst. apply aeq_abs_same. apply H. (** In the former case the result is trivial because $u =_\alpha u'$. *)
+        ** reflexivity.
+        ** assumption.
+      * intro Hneq. apply aeq_abs_diff. (** In the latter case, $x_0 \neq x_1$ and we need to prove that $\metasub{(\swap{y}{x_0}{t_1})}{x}{u} =_\alpha \swap{x_0}{x_1}{(\metasub{(\swap{y}{x_1}{t_1})}{x}{u'})}$.*)
+        ** assumption.
+        ** admit.
+        ** Abort. (** Therefore, we need to propagate the swap over the metasubstitution before been able to apply the induction hypothesis. The propagation of the swap over the metasubstitution is stated by the following lemma:
+
+%\begin{lemma} Let $t,u$ be terms, and $x,y,z$ variables. Then
+ $\swap{y}{z}{(\metasub{t}{x}{u})} =_\alpha \metasub{(\swap{y}{z}{t})}{\vswap{y}{z}{x}}{\swap{y}{z}{u}}$.
+\end{lemma}%
+
+%\noindent% whose corresponding Coq version is given by: %\newline% *)
+
+Lemma swap_m_subst: forall t u x y z, swap y z ([x := u]t) =a ([(swap_var y z x) := (swap y z u)] (swap y z t)).
+Proof.
+  induction t using n_sexp_induction. (** %\noindent{\bf Proof.}% The proof is by induction on the size of the term [t].*)
+  - intros u x' y z. unfold m_subst. rewrite subst_rec_fun_equation. destruct (x' == x) eqn:H.
+    + subst. simpl. rewrite subst_rec_fun_equation. rewrite eq_dec_refl. apply aeq_refl.
+    + simpl. apply aeq_sym. rewrite subst_rec_fun_equation. clear H. apply (swap_neq y z) in n. destruct (swap_var y z x' == swap_var y z x).
+      * contradiction.
+      * apply aeq_refl.
+  - intros u x y z'. unfold m_subst. rewrite subst_rec_fun_equation. destruct (x == z) eqn:Hxz. (** The interesting case is the abstraction, where we need to prove that $\swap{y}{z}{(\metasub{(\lambda_w.t_1)}{x}{u})} =_\alpha \metasub{(\swap{y}{z}{\lambda_w.t_1})}{\vswap{y}{z}{x}}{\swap{y}{z}{u}}$. On the left hand side, we can propagate the metasubstitution over the abstraction in the case that $x \neq w$ (the other is straighforward) and the new goal after the propagation of the swap over the abstraction is $\lambda_{\vswap{y}{z}{w'}}.\swap{y}{z}{(\metasub{\swap{w}{w'}{t_1}}{x}{u})} =_\alpha \metasub{(\lambda_{\vswap{y}{z}{w}}.\swap{y}{z}{t_1})}{\vswap{y}{z}{x}}{\swap{y}{z}{u}}$, where $w' \notin fv(\lambda_w.t_1) \cup fv(u) \cup \{x\}$.*)
+    + subst. simpl. rewrite subst_rec_fun_equation. rewrite eq_dec_refl. apply aeq_refl.
+    + destruct (atom_fresh (union (fv_nom u) (union (fv_nom (n_abs z t)) (singleton x)))). simpl. clear Hxz. pose proof n as Hxz. apply (swap_neq y z') in n. apply aeq_sym. rewrite subst_rec_fun_equation. destruct (swap_var y z' x == swap_var y z' z).
+      * contradiction.
+      * destruct (atom_fresh
+       (union (fv_nom (swap y z' u))
+          (union (fv_nom (n_abs (swap_var y z' z) (swap y z' t))) (singleton (swap_var y z' x))))). case (x1 == (swap_var y z' x0)). (** Now we propagate the metasubstitution over the abstraction in the right hand side term. Since $x\neq w$, we get $\vswap{y}{z}{x} \neq \vswap{y}{z}{w}$ and a renaming is necessary. After the renaming to a new name, say $w''$, such that $w'' \notin fv(\lambda_{\vswap{y}{z}{w}}.\swap{y}{z}{t_1}) \cup fv(\swap{y}{z}{u}) \cup \{\vswap{y}{z}{x}\}$, we get the following goal $\lambda_{\vswap{y}{z}{w'}}.\swap{y}{z}{(\metasub{\swap{w}{w'}{t_1}}{x}{u})} =_\alpha \lambda_{w''}.\metasub{(\swap{w''}{\vswap{y}{z}{w}}{(\swap{y}{z}{t_1})})}{\vswap{y}{z}{x}}{\swap{y}{z}{u}}$. We consider two cases: either $w'' = \vswap{y}{z}{w'}$ or $w'' \neq \vswap{y}{z}{w'}$.*) 
+        ** intro Heq. subst. apply aeq_abs_same. unfold m_subst in *. apply aeq_sym. rewrite <- swap_equivariance. apply H. reflexivity. 
+        ** intro Hneq. apply aeq_abs_diff.
+           *** assumption.
+           *** admit.
+           *** apply aeq_sym. unfold m_subst in H. apply aeq_trans with (swap (swap_var y z' x0) x1 (subst_rec_fun (swap y z' (swap z x0 t)) (swap y z' u) (swap_var y z' x))). (** In the former case, we can apply the rule $\mbox{\it aeq}\_\mbox{\it abs}\_\mbox{\it same}$ and we get $\swap{y}{z}{(\metasub{(\swap{w}{w'}{t_1})}{x}{u})} =_\alpha \metasub{(\swap{w''}{\vswap{y}{z}{w}}{(\swap{y}{z}{t_1})})}{\vswap{y}{z}{x}}{\swap{y}{z}{u}}$ that can be proved by the induction hypothesis.*)
+               **** apply aeq_swap. rewrite H.
+                    ***** apply aeq_refl. Abort. (** When $w'' \neq \vswap{y}{z}{w'}$, the application of the rule $\mbox{\it aeq}\_\mbox{\it abs}\_\mbox{\it diff}$ generates the goal $\swap{w''}{\vswap{y}{z}{w'}}{\swap{y}{z}{(\metasub{\swap{w}{w'}{t_1}}{x}{u})}} =_\alpha \metasub{(\swap{w''}{\vswap{y}{z}{w}}{(\swap{y}{z}{t_1})})}{\vswap{y}{z}{x}}{\swap{y}{z}{u}}$. We can use the induction hypothesis to propagate the swap inside the metasubstitution, and then we get an $\alpha$-equality with metasubstitution as main operation on both sides, and whose correspondent components are $\alpha$-equivalent. In a more abstract way, we have to prove an $\alpha$-equality of the form $\metasub{t}{x}{u} =_\alpha \metasub{t'}{x}{u'}$, where $t =_\alpha t'$ and $u =_\alpha u'$. The problem is that we cannot rewrite $\alpha$-equalities inside metasubstitution unless we prove some special lemmas stating the compatibilities between them using the [Equations] library or something similar. Alternatively, if we decide to analise the metasubtitution componentwise, %{\it i.e.}% as stated in a lemma similar to [aeq_m_subst_in_trial], we get a circular proof problem because both [aeq_m_subst_in_trial] and [swap_m_subst] depend on each other to be proved. We will present a solution that do not use any additional library, but it adds the following axiom to the formalization:*)
+                  
+Axiom Eq_implies_equality: forall s s': atoms, s [=] s' -> s = s'.
+
+(** This axiom transform a set equality into a syntactic equality. This will allow us to rewrite sets of atoms in a more flexible way. To show how it works, we will start proving the lemma [aeq_m_subst_in] without the need of the lemma [swap_m_subst]:*)
 
 Lemma aeq_m_subst_in: forall t u u' x, u =a u' -> ([x := u] t) =a ([x := u'] t).
 Proof.
-  induction t using n_sexp_induction.
+  induction t using n_sexp_induction. (** %\noindent{\bf Proof.}% The proof is by induction on the size of the term [t].*)
   - intros u u' x' Haeq. pose proof Haeq as Hfv. apply aeq_fv_nom in Hfv. apply Eq_implies_equality in Hfv. unfold m_subst in *. repeat rewrite subst_rec_fun_equation. destruct (x' == x).
     + assumption.
-    + reflexivity.
-  - intros u u' x Haeq. pose proof Haeq as Hfv. apply aeq_fv_nom in Hfv. apply Eq_implies_equality in Hfv. unfold m_subst in *. repeat rewrite subst_rec_fun_equation. rewrite Hfv. destruct (atom_fresh (union (fv_nom u') (union (fv_nom (n_abs z t)) (singleton x)))). destruct (x == z).
+    + reflexivity. 
+  - intros u u' x Haeq. pose proof Haeq as Hfv. apply aeq_fv_nom in Hfv. apply Eq_implies_equality in Hfv. unfold m_subst in *. repeat rewrite subst_rec_fun_equation. rewrite Hfv. destruct (atom_fresh (union (fv_nom u') (union (fv_nom (n_abs z t)) (singleton x)))). destruct (x == z). (** The interesting case is the abstraction. We have by hypothesis that $u =_\alpha u'$ therefore both $u$ and $u'$ have the same set of free variables by lemma [aeq_fv_nom]. With the axiom [Eq_implies_equality], we can replace the set $fv(u)$ by $fv(u')$, or vice-versa, in such a way that instead of generating two new names for the propagation of the metasusbstitutions inside the abstractions, we need just one new name and there is no more the case where the binders of the abstractions were different names. *)
       * apply aeq_refl.
       * apply aeq_abs_same. apply H.
         ** reflexivity.
@@ -2525,7 +1886,7 @@ Proof.
   - intros u u' x Haeq. unfold m_subst in *. rewrite subst_rec_fun_equation. apply aeq_sym. rewrite subst_rec_fun_equation. apply aeq_app.
     + apply IHt1. apply aeq_sym. assumption.
     + apply IHt2. apply aeq_sym. assumption.
-  - intros u u' x Haeq. unfold m_subst in *. rewrite subst_rec_fun_equation. apply aeq_sym. rewrite subst_rec_fun_equation. pose proof Haeq as Hfv. apply aeq_fv_nom in Hfv. apply Eq_implies_equality in Hfv. rewrite Hfv. destruct (atom_fresh (union (fv_nom u') (union (fv_nom (n_sub t1 z t2)) (singleton x)))). destruct (x == z).
+  - intros u u' x Haeq. unfold m_subst in *. rewrite subst_rec_fun_equation. apply aeq_sym. rewrite subst_rec_fun_equation. pose proof Haeq as Hfv. apply aeq_fv_nom in Hfv. apply Eq_implies_equality in Hfv. rewrite Hfv. destruct (atom_fresh (union (fv_nom u') (union (fv_nom (n_sub t1 z t2)) (singleton x)))). destruct (x == z). (** The case of the explicit substitution is similar, and with this strategy we avoid the rules $\mbox{\it aeq}\_\mbox{\it abs}\_\mbox{\it diff}$ and $\mbox{\it aeq}\_\mbox{\it sub}\_\mbox{\it diff}$ that introduce swappings. $\hfill\Box$*)
     + apply aeq_sub_same.
       * apply aeq_refl.
       * apply IHt1. apply aeq_sym. assumption.
@@ -2534,10 +1895,9 @@ Proof.
         ** reflexivity.
         ** apply aeq_sym. assumption.
       * apply IHt1. apply aeq_sym. assumption.
-Qed.
-
+Qed. (** %\newline% *)
+       
 (* begin hide *)
-
 Lemma aeq_abs_notin: forall t1 t2 x y, x <> y ->  n_abs x t1 =a n_abs y t2 -> x `notin` fv_nom t2.
 Proof.
   intros t1 t2 x y Hneq Haeq. inversion Haeq; subst.
@@ -2551,71 +1911,56 @@ Proof.
   - contradiction.
   - assumption.
 Qed.
-
 (* end hide *)
 
-(** The next lemma states that if the meta-substitution in both sides of an alpha-equivalency is the same and the expression the meta-substition is applied to are different, then the expressions outside the meta-substitions have to be alpha-equivalent in both sides.**)
-(** The proof for this lemma is done on induction in the expression, generating one case for each of the possible expressions and the definition of the meta-substitution is used to complete the proof. In the case of the variable, the proof is trivial. **)
-(** In the abstraction, we use the technique of comparing the variables of the meta-substitution and the one for the abstraction. **)
-(** The apllication case is also trivial. **)
-(** In the explicit substitution case, we have that the left side of the substitution generates a case similar to the one of the abstraction and the right side generates one similar to the one in the application.**)
-
-
+(** The next lemma, named [aeq_m_subst_out] will benefit the strategy used in the previous proof, but it is not straightfoward. In the proof below, we will mostly use Coq notation, instead of the metanotation of the previous proof. We believe that at this point of the work, even the readers not familiar with Coq, can easily understand the Coq code interleaved with metanotation. *)
 Lemma aeq_m_subst_out: forall t t' u x, t =a t' -> ([x := u] t) =a ([x := u] t').
 Proof.
-  induction t using n_sexp_induction.
+  induction t as [y | t1 y | t1 t2 | t1 y t2] using n_sexp_induction . (** %\noindent{\bf Proof.}% The proof is by induction on the size of the term [t]. *)
   - intros t' u x' Haeq. inversion Haeq; subst. apply aeq_refl.
-  - intros t' u x Haeq. inversion Haeq; subst.
-    + pose proof Haeq as Hfv. apply aeq_fv_nom in Hfv. simpl in *. apply Eq_implies_equality in Hfv. unfold m_subst in *. repeat rewrite subst_rec_fun_equation. simpl. rewrite Hfv. destruct (atom_fresh (union (fv_nom u) (union (remove z (fv_nom t2)) (singleton x)))). destruct (x == z).
+  - intros t' u x Haeq. inversion Haeq; subst. (** The interesting case is the abstraction. The are two cases based on the definition of the $\alpha$-equivalence relation: either the binders have the same name or they are different. *)
+    + pose proof Haeq as Hfv. apply aeq_fv_nom in Hfv. simpl in *. apply Eq_implies_equality in Hfv. unfold m_subst in *. repeat rewrite subst_rec_fun_equation. simpl. rewrite Hfv. destruct (atom_fresh (union (fv_nom u) (union (remove y (fv_nom t2)) (singleton x)))). destruct (x == y). (** In the former case, we have to prove [ ([x := u] n_abs y t1) =a ([x := u] n_abs y t2)] assumming that [t1 =a t2]. In both sides of the $\alpha$-equation, the metasubstitutition need to be propagated over the abstraction, and according to our definition of metasubstitution, one name will be generated for each propagation. The new name to be generate for the term [[x := u] (n_abs y t1)] (lhs) is such that it is not in the set $fv(\lambda_y.t_1)\cup fv(u) \cup \{x\}$, while the new name to be generated for the term [[x := u] (n_abs y t2)] (rhs) is such that it is not in the set $fv(\lambda_y.t_2)\cup fv(u) \cup \{x\}$. Since [t1 =a t2], by lemma [aeq_fv_nom] the set of free variables of [t1] is equal to the set of free variables of [t2], and therefore, we can generate just one new name for both propagations of the metasubstitution. *)
       * assumption.
-      * apply aeq_abs_same. apply H.
+      * apply aeq_abs_same. apply H. (** If this new name is [x0] then the new goal to be proved is [n_abs x0 (subst_rec_fun (swap y x0 t1) u x) =a n_abs x0 (subst_rec_fun (swap y x0 t2) u x)], which can be proved by the induction hypothesis. *)
         ** reflexivity.
         ** apply aeq_swap. assumption.
-    + pose proof Haeq as Hfv. apply aeq_fv_nom in Hfv. simpl in *. apply Eq_implies_equality in Hfv. unfold m_subst in *. rewrite subst_rec_fun_equation. simpl. apply aeq_sym. rewrite subst_rec_fun_equation. simpl. rewrite Hfv. destruct (atom_fresh (union (fv_nom u) (union (remove y (fv_nom t2)) (singleton x)))). destruct (x == y).
-      * subst. destruct (y == z).
-        ** symmetry in e. contradiction.
-        ** rewrite <- Haeq. pose proof n as Hnotin. repeat apply notin_union_2 in n. apply notin_singleton_1 in n. case (z == x0).
-           *** intro Heq. subst.  apply aeq_abs_same. rewrite swap_id. apply aeq_sym in Haeq. apply aeq_abs_notin in Haeq.
-               **** apply aeq_sym. apply m_subst_notin. assumption.
-               ****assumption.
-           *** intro Hneq. apply aeq_abs_diff.
+    + pose proof Haeq as Hfv. apply aeq_fv_nom in Hfv. simpl in *. apply Eq_implies_equality in Hfv. unfold m_subst in *. case (y == x).
+      * intro Heq. subst. rewrite subst_rec_fun_equation. rewrite eq_dec_refl. rewrite subst_rec_fun_equation. destruct (x == y0). (** If [y = x] then [x <> y0] and the metasubstitution [[x := u]] has no effect on the LHS, but it can be propagated on the RHS, %{\it i.e.}% over the abstraction [(n_abs y0 t2)] but it also has no effect in [t2] because [x] does not occur free in [t2]. *)
+        ** contradiction.
+        ** destruct (atom_fresh (union (fv_nom u) (union (fv_nom (n_abs y0 t2)) (singleton x)))). apply aeq_trans with (n_abs x0 (swap y0 x0 t2)).
+           *** apply aeq_trans with (n_abs y0 t2).
                **** assumption.
-               **** apply aeq_sym in Haeq. apply aeq_abs_notin in Haeq. assert (Hsub: subst_rec_fun (swap z x0 t) u y =a swap z x0 t).
-                    ***** apply m_subst_notin. apply fv_nom_remove_swap; assumption.
-                    ***** apply aeq_fv_nom in Hsub. rewrite Hsub. apply fv_nom_swap. rewrite <- Hfv in Hnotin. apply notin_union_2 in  Hnotin. apply notin_union_1 in Hnotin. apply notin_remove_1 in Hnotin. destruct Hnotin.
-                    ****** contradiction.
-                    ****** assumption.
-                    ***** assumption.
-               **** apply aeq_sym in Haeq. apply aeq_abs_notin in Haeq. rewrite (swap_symmetric _ z x0). apply aeq_trans with (swap x0 z (swap x0 z t)).
-                    ***** rewrite swap_involutive. apply aeq_refl.
-                    ***** apply aeq_swap. apply aeq_sym. apply m_subst_notin. apply fv_nom_remove_swap; assumption.
-                    ***** assumption.
-      * destruct (x == z).
-        ** rewrite Haeq. subst. case (x0 == y). 
-           *** intro Heq. subst. apply aeq_abs_same. rewrite swap_id. apply m_subst_notin. assumption.
-           *** intro Hneq. apply aeq_abs_diff. 
-               **** assumption.
-               **** apply notin_union_2 in n. apply notin_union_1 in n. apply notin_remove_1 in n. destruct n.
-                    ***** symmetry in H0. contradiction.
-                    ***** assumption.
-               **** apply m_subst_notin. apply fv_nom_remove_swap. 
-                    ****** repeat apply notin_union_2 in n. apply notin_singleton_1 in n. assumption.
-                    ****** assumption.
-                    ****** assumption.
-        ** apply aeq_abs_same. apply H.
-           *** apply aeq_size in H5. rewrite swap_size_eq in H5. auto.
-           *** case (x0 == y).
-               **** intro Heq. subst. rewrite swap_id. apply (aeq_swap _ _ y z) in H5. rewrite swap_involutive in H5. apply aeq_sym. rewrite (swap_symmetric _ z y). assumption.
-               **** intro Hneq. apply aeq_sym. apply (aeq_swap _ _ z x0) in H5. rewrite H5. rewrite (swap_symmetric _ z x0). rewrite (swap_symmetric _ y z). rewrite (swap_symmetric _ y x0). apply aeq_swap_swap.
-                    ***** apply notin_union_2 in n. apply notin_union_1 in n. apply notin_remove_1 in n. destruct n.
+               **** case (x0 == y0).
+                    ***** intro Heq. subst. rewrite swap_id. apply aeq_refl.
+                    ***** intro Hneq. pose proof n0 as Hx0. apply notin_union_2 in n0. apply notin_union_1 in n0. simpl in n0. apply notin_remove_1 in n0. destruct n0.
                     ****** symmetry in H0. contradiction.
-                    ****** assumption.
-                    ***** assumption.
+                    ****** apply aeq_abs_diff.
+                    ******* apply aux_not_equal. assumption.
+                    ******* apply fv_nom_swap. assumption.
+                    ******* rewrite (swap_symmetric _ y0 x0). rewrite swap_involutive. apply aeq_refl.
+           *** apply aeq_abs_same. apply aeq_sym. apply m_subst_notin. repeat apply notin_union_2 in n0. apply notin_singleton_1 in n0. apply fv_nom_remove_swap; assumption. 
+      * intro Hneq. case (y0 == x). (** If [y <> x] then the metasubstitution can be propagated over the abstraction of the LHS, and similarly we compare [x] with [y0] to see what happens in the RHS. *)
+        ** intro Heq. apply aeq_sym in Haeq. apply aeq_abs_notin in Haeq.
+           *** symmetry in Heq. subst. apply aeq_sym. rewrite subst_rec_fun_equation. rewrite eq_dec_refl. apply aeq_sym. apply aeq_trans with (n_abs y t1).
+               **** apply m_subst_notin. simpl. apply notin_remove_2. assumption.
+               **** apply aeq_abs_diff; assumption. (** When [y0 = x] then the metasubstitution has no effect on the abstraction of the RHS. On the LHS the metasubstitution is propagated since [y <> x] but, as in the previous case, it has no effect in [t1] because [y0] does not occur free in [t1].*)
+           *** apply aux_not_equal. assumption.
+        ** intro Hneq'. repeat rewrite subst_rec_fun_equation. simpl. rewrite Hfv. destruct (atom_fresh (union (fv_nom u) (union (remove y0 (fv_nom t2)) (singleton x)))). destruct (x == y). (** Now we have to prove that [[x := u](n_abs y t1) =a [x := u](n_abs y0 t2)], when [y <> x], [y0 <> x] and [n_abs y t1 =a n_abs y0 t2]. Since the set of free variables of [n_abs y t1] is equal to the set of free variables of [n_abs y0 t2], we can as in the previous case generate only one new name, say [x0] that fulfill the condition to propagate the metasubstitution on both sides of the $\alpha$-equation. More precisely, $x_0 \notin fv(\lambda_y.t1) \cup fv(u) \cup \{x\}$, and the goal to be proved is [n_abs x0 ([x := u](swap y x0 t1)) =a n_abs x0 ([x := u](swap y0 x0 t2))].*)
+           *** symmetry in e. contradiction.
+           *** destruct (x == y0).
+               **** symmetry in e. contradiction.
+               **** apply  aeq_abs_same. apply H. (** As just one new name was generated, there is no case where the binders of the abstractions are different. Remember that abstractions with different binders were the cause of the circularity problem in the proofs because the application of the rule [aeq_abs_diff] introduces a new swap that will be outside the metasubstitution in this case, whose solution would require a lemma of the form of [swap_m_subst]. Therefore, after an applycation of the rule [aeq_abs_same], we conclude with the induction hypothesis.*)
+                    ***** reflexivity.
+                    ***** apply (aeq_swap _ _ y x0) in H5. rewrite H5. case (x0 == y0).
+                    ****** intro Heq. subst. rewrite swap_id. rewrite (swap_symmetric _ y y0). rewrite swap_involutive. apply aeq_refl.
+                    ****** intro Hneq''. rewrite (swap_symmetric _ y x0). rewrite (swap_symmetric _ y0 y). rewrite (swap_symmetric _ y0 x0). apply notin_union_2 in n. apply notin_union_1 in n. apply notin_remove_1 in n. destruct n.
+                    ******* symmetry in H0. contradiction.
+                    ******* apply aeq_swap_swap; assumption.
   - intros t u x Haeq. inversion Haeq; subst. clear Haeq. unfold m_subst in *. rewrite subst_rec_fun_equation. apply aeq_sym. rewrite subst_rec_fun_equation. apply aeq_app.
-    + apply aeq_sym. apply IHt1. assumption.
     + apply aeq_sym. apply IHt2. assumption.
-  - intros t u x Haeq. inversion Haeq; subst.
-    + unfold m_subst in *. rewrite subst_rec_fun_equation. apply aeq_sym. rewrite subst_rec_fun_equation. apply aeq_fv_nom in Haeq. apply Eq_implies_equality in Haeq. rewrite Haeq. destruct (atom_fresh (union (fv_nom u) (union (fv_nom (n_sub t1' z t2')) (singleton x)))). simpl in *. destruct (x == z).
+    + apply aeq_sym. apply IHt1. assumption.
+  - intros t u x Haeq. inversion Haeq; subst. (** The explicit substitution operation is also interesting, but the proof strategy is similar to the one used in the abstraction case. $\hfill\Box$*)
+    + unfold m_subst in *. rewrite subst_rec_fun_equation. apply aeq_sym. rewrite subst_rec_fun_equation. apply aeq_fv_nom in Haeq. apply Eq_implies_equality in Haeq. rewrite Haeq. destruct (atom_fresh (union (fv_nom u) (union (fv_nom (n_sub t1' t2 t2')) (singleton x)))). simpl in *. destruct (x == t2).
       * apply aeq_sub_same.
         ** apply aeq_sym. assumption.
         ** apply aeq_sym. apply IHt1. assumption.
@@ -2624,8 +1969,8 @@ Proof.
            *** reflexivity.
            *** apply aeq_swap. assumption.
         ** apply aeq_sym. apply IHt1. assumption.
-    + unfold m_subst in *. rewrite subst_rec_fun_equation. apply aeq_sym. rewrite subst_rec_fun_equation. pose proof Haeq as Hfv. apply aeq_fv_nom in Hfv. apply Eq_implies_equality in Hfv. rewrite Hfv. destruct (atom_fresh (union (fv_nom u) (union (fv_nom (n_sub t1' y t2')) (singleton x)))). destruct (x == y).
-      * subst. destruct (y == z).
+    + unfold m_subst in *. rewrite subst_rec_fun_equation. apply aeq_sym. rewrite subst_rec_fun_equation. pose proof Haeq as Hfv. apply aeq_fv_nom in Hfv. apply Eq_implies_equality in Hfv. rewrite Hfv. destruct (atom_fresh (union (fv_nom u) (union (fv_nom (n_sub t1' y0 t2')) (singleton x)))). destruct (x == y0).
+      * subst. destruct (y0 == t2).
         ** subst. contradiction.
         ** pose proof n as Hx0. repeat apply notin_union_2 in n. apply notin_singleton_1 in n. apply aeq_sym. apply aeq_sub_diff.
            *** apply IHt1. assumption.
@@ -2633,43 +1978,44 @@ Proof.
            *** apply notin_union_2 in Hx0. apply notin_union_1 in Hx0. simpl in Hx0. apply notin_union_1 in Hx0. apply notin_remove_1 in Hx0. destruct Hx0.
                **** contradiction.
                ****assumption.
-           *** apply aeq_trans with (swap z x0 t1).
+           *** apply aeq_trans with (swap t2 x0 t1).
                **** apply m_subst_notin. apply aeq_sym in Haeq. apply aeq_sub_notin in Haeq.
                     ***** apply fv_nom_remove_swap.
                     ****** assumption.
                     ****** apply aux_not_equal. assumption.
                     ****** assumption.
                     ***** assumption.
-               **** apply aeq_trans with (swap z x0 (swap y z t1')).
+               **** apply aeq_trans with (swap t2 x0 (swap y0 t2 t1')).
                     ***** apply aeq_swap. assumption.
-                    ***** rewrite (swap_symmetric _ z x0). rewrite (swap_symmetric _ y z). rewrite (swap_symmetric _ y x0). apply aeq_swap_swap.
+                    ***** rewrite (swap_symmetric _ t2 x0). rewrite (swap_symmetric _ y0 t2). rewrite (swap_symmetric _ y0 x0). apply aeq_swap_swap.
                     ****** apply notin_union_2 in Hx0. apply notin_union_1 in Hx0. simpl in Hx0. apply notin_union_1 in Hx0. apply notin_remove_1 in Hx0. destruct Hx0.
                     ******* contradiction.
                     ******* assumption.
                     ****** assumption.
-      * destruct (x == z).
+      * destruct (x == t2).
         ** subst. pose proof n as Hx0. repeat apply notin_union_2 in n. apply notin_singleton_1 in n. apply aeq_sub_diff.
            *** apply aeq_sym. apply IHt1. assumption.
            *** apply aux_not_equal. assumption.
            *** rewrite <- Hfv in Hx0. apply notin_union_2 in Hx0. apply notin_union_1 in Hx0. simpl in Hx0. apply notin_union_1 in Hx0. apply notin_remove_1 in Hx0. destruct Hx0.
                **** contradiction.
                **** assumption.
-           *** apply aeq_trans with (swap y x0 t1').
-               **** apply m_subst_notin. apply fv_nom_remove_swap; assumption.
-               **** rewrite <- Hfv in Hx0. apply (aeq_swap1  _ _ y z) in H7. rewrite swap_involutive in H7. apply aeq_sym in H7. apply (aeq_swap1 _ _ y x0) in H7. rewrite H7. rewrite (swap_symmetric _ y x0). rewrite (swap_symmetric _ z x0). apply aeq_swap_swap.
-                    ****** apply notin_union_2 in Hx0. apply notin_union_1 in Hx0. simpl in Hx0. apply notin_union_1 in Hx0. apply notin_remove_1 in Hx0. destruct Hx0.
-                    ******* contradiction.
+           *** case (x0 == y0). 
+               **** intro Heq. subst. rewrite swap_id. apply aeq_trans with t1'.
+                    ***** apply m_subst_notin. assumption.
+                    ***** apply (aeq_swap _ _ t2 y0) in H7. rewrite H7. rewrite (swap_symmetric _ t2 y0). rewrite swap_involutive. apply aeq_refl.
+               **** intro Hneq. apply aeq_trans with (swap y0 x0 t1').
+                    ***** apply m_subst_notin. apply fv_nom_remove_swap; assumption.
+                    ***** apply (aeq_swap _ _ t2 x0) in H7. rewrite H7. apply aeq_sym. rewrite (swap_symmetric _ t2 x0). rewrite (swap_symmetric _ y0 t2). rewrite (swap_symmetric _ y0 x0). apply aeq_swap_swap.
+                    ******  apply notin_union_2 in Hx0. apply notin_union_1 in Hx0. simpl in Hx0. apply notin_union_1 in Hx0. apply notin_remove_1 in Hx0. destruct Hx0.
+                    ******* symmetry in H0. contradiction.
                     ******* assumption.
-                    ****** apply aeq_sym in Haeq. apply aeq_sub_notin in Haeq.
-                    ******* assumption.
-                    ******* apply aux_not_equal. assumption.
+                    ****** assumption.
         ** apply aeq_sub_same.
            *** apply H.
                **** apply aeq_size in H7. symmetry. rewrite swap_size_eq in H7. assumption.
-               **** case (x0 == y). 
-                    ***** intro Heq. subst. rewrite swap_id. rewrite (swap_symmetric _ z y). apply (aeq_swap1 _ _ y z) in H7.
-                    rewrite H7. rewrite swap_involutive. apply aeq_refl.
-                    ***** intro Hneq. apply (aeq_swap1 _ _ z x0) in H7. rewrite H7. apply aeq_sym. rewrite (swap_symmetric _ z x0). rewrite (swap_symmetric _ y z). rewrite (swap_symmetric _ y x0). apply aeq_swap_swap.
+               **** case (x0 == y0). 
+                    ***** intro Heq. subst. rewrite swap_id. apply (aeq_swap1 _ _ y0 t2) in H7. rewrite (swap_symmetric _ t2 y0). rewrite H7. rewrite swap_involutive. apply aeq_refl.
+                    ***** intro Hneq. apply (aeq_swap1 _ _ t2 x0) in H7. rewrite H7. apply aeq_sym. rewrite (swap_symmetric _ t2 x0). rewrite (swap_symmetric _ y0 t2). rewrite (swap_symmetric _ y0 x0). apply aeq_swap_swap.
                     ****** apply notin_union_2 in n. apply notin_union_1 in n. simpl in n. apply notin_union_1 in n. apply notin_remove_1 in n. destruct n.
                     ******* symmetry in H0. contradiction.
                     ******* assumption.
@@ -2677,8 +2023,8 @@ Proof.
            *** apply aeq_sym. apply IHt1. assumption.
 Qed.
 
-(** The corollary bellow states that if the variable is the same in two meta substitutions, they are alpha-equivalent if the other terms are alpha-equivalent, respectively. The proof of this corollary is done using both lemmas above to show the equality amongst the terms.**)
-          
+(** As a corollary, one can join the lemmas [aeq_m_subst_in] and [aeq_m_subst_out] as follows:*)
+
 Corollary aeq_m_subst_eq: forall t t' u u' x, t =a t' -> u =a u' -> ([x := u] t) =a ([x := u'] t').
 Proof.
   intros t t' u u' x H1 H2. apply aeq_trans with ([x:=u]t').
@@ -2686,221 +2032,138 @@ Proof.
   - apply aeq_m_subst_in. assumption.
 Qed.
 
-
-(** The following lemma states that a swap can be propagated inside the metasubstitution resulting in an $\alpha$-equivalent term. *)
+(** Now, we show how to propagated a swap inside metasubstitutions using the decomposition of the metasubstitution provided by the corollary [aeq_m_subst_eq].%\newline% *)
 
 Lemma swap_subst_rec_fun: forall x y z t u, swap x y (subst_rec_fun t u z) =a subst_rec_fun (swap x y t) (swap x y u) (swap_var x y z).
 Proof.
-
-  (** Firstly, we compare [x] and [y] which gives a trivial case when they are the same. *)
+  (** %\noindent{\bf Proof.}% Firstly, we compare [x] and [y], since the case [x = y] is trivial.*)
   intros x y z t u. destruct (x == y). 
   - subst. repeat rewrite swap_id. rewrite swap_var_id. apply aeq_refl.
-    (** In this way, we can assume in the rest of the proof that [x] and [y] are different from each other. The proof proceeds by induction on the size of the term [t]. The tricky case is the abstraction and substitution cases. *)
-  - generalize dependent u. generalize dependent z. generalize dependent y. generalize dependent x.
-    induction t using n_sexp_induction.
-    
-    + intros x' y Hneq z u. rewrite subst_rec_fun_equation. destruct (z == x).
+    (** The proof proceeds by induction on the size of the term [t], assuming that [x <> y]. The tricky cases are the abstraction and explicit substitution. *)
+  - generalize dependent u. generalize dependent z. generalize dependent y. generalize dependent x. induction t as  [y | t1 y | t1 t2 | t1 t2 y] using n_sexp_induction.    
+    + intros x' y' Hneq z u. rewrite subst_rec_fun_equation. destruct (z == y).
       * subst. simpl swap at 2. rewrite subst_rec_fun_equation. rewrite eq_dec_refl. apply aeq_refl.
-      * pose proof swap_neq as Hswap. specialize (Hswap x' y z x). apply Hswap in n; clear Hswap.
-        simpl swap at 2. rewrite subst_rec_fun_equation. destruct (swap_var x' y z == swap_var x' y x).
+      * pose proof n as Hswap. apply (swap_neq x' y') in n. simpl swap at 2. rewrite subst_rec_fun_equation. destruct (swap_var x' y' z == swap_var x' y' y).
         ** contradiction.
         ** simpl swap. apply aeq_refl.
-    + intros x y Hneq z' u. rewrite subst_rec_fun_equation. case (z' == z).
-      * intro Heq. subst. simpl. rewrite subst_rec_fun_equation. rewrite eq_dec_refl. apply aeq_refl.
-      * intro Hneq'. simpl in *. rewrite subst_rec_fun_equation. destruct (swap_var x y z' == swap_var x y z).
-        ** apply (swap_neq x y) in Hneq'. contradiction.
-        ** simpl. destruct (atom_fresh (union (fv_nom u) (union (remove z (fv_nom t)) (singleton z')))). destruct (atom_fresh (union (fv_nom (swap x y u)) (union (remove (swap_var x y z) (fv_nom (swap x y t))) (singleton (swap_var x y z'))))). simpl. apply aeq_trans with (n_abs (swap_var x y x0) (subst_rec_fun (swap x y (swap z x0 t)) (swap x y u) (swap_var x y z'))).
-           *** apply aeq_abs_same. apply H. 
-               **** reflexivity.
-               **** assumption.
-           *** case (x1 == swap_var x y x0). 
-               **** intro Heq. subst. apply aeq_abs_same. apply aeq_m_subst_out. rewrite swap_equivariance. apply aeq_refl.
-               **** intro Hneq''. rewrite (swap_equivariance _ x y z x0). apply aeq_abs_diff. 
+    + intros x y' Hneq z u. simpl. case (y == z). (** In the abstraction case, %{\it i.e.}% when $t = \lambda_{y'}.t_1$ then we must prove that [swap x y ([z := u](n_abs y' t1)) =a [(swap_var x y z) := (swap x y u)](swap x y (n_abs y' t1))], and the induction hypothesis states that a swap can be propagated inside a metasubstitution whose body is a term with the same size as [t1]. Firstly, we compare the variables [y'] and [z] to check whether we should propagate the metasubstitution inside the abstraction of the LHS. *)
+      * intro Heq. subst. repeat rewrite subst_rec_fun_equation. repeat rewrite eq_dec_refl. simpl. apply aeq_refl. (** When [y' = z] the metasubstitution is erased according to the definition %(\ref{msubst})% on both sides of the $\alpha$-equation and we are done.*)
+      * intro Hneq'. repeat rewrite subst_rec_fun_equation. destruct (z == y). (** When [y' <> z] then the metasubstitutions on both sides of the $\alpha$-equation need to be propagated inside the corresponding abstractions. In order to do so, a new name need to be created. Note that in this case, it is not possible to create a unique name for both sides because the name of the LHS cannot belong to the set $fv(\lambda_y'.t_1) \cup fv(u) \cup \{z\}$, while the name of the RHS cannot belong to the set $fv(\swap{x}{y}{\lambda_y'.t_1}) \cup fv(\swap{x}{y}{u}) \cup \{\vswap{x}{y}{z}\}$.*)
+        ** symmetry in e. contradiction.
+        ** destruct (swap_var x y' z == swap_var x y' y).
+           *** apply (swap_neq x y') in n. contradiction.
+           *** simpl. destruct (atom_fresh (union (fv_nom u) (union (remove y (fv_nom t1)) (singleton z)))). destruct (atom_fresh (union (fv_nom (swap x y' u)) (union (remove (swap_var x y' y) (fv_nom (swap x y' t1))) (singleton (swap_var x y' z))))). simpl. case (x1 == swap_var x y' x0). (** Let [x0] be a new name that is not in the set $fv(\lambda_y'.t_1) \cup fv(u) \cup \{z\}$, and [x1] a new name that is not in the set $fv(\swap{x}{y}{\lambda_y'.t_1}) \cup fv(\swap{x}{y}{u}) \cup \{\vswap{x}{y}{z}\}$. After renaming and propagating the metasubstitutions inside the abstractions, the current goal is [n_abs (swap_var x y x0) (swap x y ([z := u](swap y' x0 t1))) =a n_abs x1 ([(swap_var x y z) := (swap x y u)](swap (swap_var x y y') x1 (swap x y t1)))]. We proceed by comparing [x1] with [(swap_var x y x0)].*)
+               **** intro Heq. subst. apply aeq_abs_same. rewrite H. rewrite <- swap_equivariance. apply aeq_refl. (** If [x1 = (swap_var x y x0)] then we use the induction hypothesis to propagate the swap inside the metasubstitution in the LHS and the current goal is [[(swap_var x y z) := (swap x y u)](swap x y (swap y' x0 t1)) =a
+  [(swap_var x y z) := (swap x y u)](swap (swap_var x y y') (swap_var x y x0) (swap x y t1))] that is proved by the swap equivariance lemma [swap_equivariance].*)
+               ***** reflexivity.
+               ***** assumption.
+               **** intro Heq''. apply aeq_abs_diff. (** If [x1 <> (swap_var x y x0)] then by the rule [aeq_abs_diff] we have to prove that the variable [swap_var x y x0] is not in the set of free variables of the term [[(swap_var x y z) := (swap x y u)](swap (swap_var x y y') x1 (swap x y t1))] and that [swap x y ([z := u](swap y' x0 t1)) =a
+  swap x1 (swap_var x y' x0) ([(swap_var x y z) := (swap x y' u)](swap (swap_var x y' y) x1 (swap x y' t1)))].*)
                     ***** apply aux_not_equal. assumption.
                     ***** apply fv_nom_remove.
-                    ****** apply notin_union_1 in n0. apply notin_fv_nom_equivariance. assumption.
-                    ****** apply notin_remove_2. pose proof n0 as Hx0. apply notin_union_2 in n0. apply notin_union_1 in n0. apply notin_remove_1 in n0. case (z == x0).
-                    ******** intro Heq. subst. apply fv_nom_swap. apply notin_union_2 in n1. apply notin_union_1 in n1. apply notin_remove_1 in n1. destruct n1.
+                    ****** apply notin_fv_nom_equivariance. apply notin_union_1 in n1. assumption.
+                    ****** apply notin_remove_2. pose proof n1 as Hx0. case (y == x0).
+                    ******** intro Heq. subst. apply fv_nom_swap. apply notin_union_2 in n2. apply notin_union_1 in n2. apply notin_remove_1 in n2. destruct n2.
                     ********* symmetry in H0. contradiction.
                     ********* assumption.
                     ******** intros Hneq'''. apply fv_nom_remove_swap.
                     ********* apply aux_not_equal. assumption.
                     ********* apply aux_not_equal. apply swap_neq. assumption.
-                    ********* destruct n0.
+                    ********* apply notin_union_2 in n1. apply notin_union_1 in n1. apply notin_remove_1 in n1. destruct n1.
                     ********** contradiction.
-                    ********** apply notin_fv_nom_equivariance. assumption.
-                    ***** rewrite H.
-                    ****** replace (swap_var x1 (swap_var x y x0) (swap_var x y z')) with (swap_var x y z').
-                    ******* apply aeq_m_subst_eq.
-                    ******** apply notin_union_2 in n0. apply notin_union_1 in n0. apply notin_remove_1 in n0. destruct n0. 
-                    *********** subst. repeat rewrite swap_id. rewrite (swap_symmetric _ x1 (swap_var x y x0)). rewrite swap_involutive. apply aeq_refl.
-                    *********** apply notin_union_2 in n1. apply notin_union_1 in n1. apply notin_remove_1 in n1. destruct n1.
-                    ************ subst. rewrite swap_id. apply aeq_refl.
-                    ************ apply aeq_sym. rewrite (swap_symmetric _ x1 (swap_var x y x0)). rewrite (swap_symmetric _ (swap_var x y z) x1). pose proof aeq_swap_swap as Hswap. specialize (Hswap (swap x y t) x1 (swap_var x y z) (swap_var x y x0)). rewrite (swap_symmetric _ (swap_var x y z) (swap_var x y x0)). apply Hswap.
-                    ************* apply notin_fv_nom_equivariance. assumption.
-                    ************* assumption.
-                    ******** apply aeq_sym. apply swap_reduction.
-                    ********* apply notin_union_1 in n1. assumption.
-                    ********* apply notin_union_1 in n0. apply notin_fv_nom_equivariance. assumption.
-                    ******* symmetry. unfold swap_var at 1. destruct (swap_var x y z' ==  x1).
-                    ******** repeat apply notin_union_2 in n1. apply notin_singleton_1 in n1. contradiction.
-                    ******** destruct (swap_var x y z' == swap_var x y x0).
-                    ********* repeat apply notin_union_2 in n0. apply notin_singleton_1 in n0. apply (swap_neq x y) in n0. contradiction.
-                    ********* reflexivity.
-                    ****** apply swap_size_eq.
-                    ****** assumption.
-    + intros x y H z u. rewrite subst_rec_fun_equation. simpl. apply aeq_sym. rewrite subst_rec_fun_equation. apply aeq_sym. apply aeq_app.
-      * apply IHt1. assumption.
-      * apply IHt2. assumption.
-    + intros x y Hneq z' u. simpl. rewrite subst_rec_fun_equation. destruct (z' == z).
-      * subst. simpl. apply aeq_sym. rewrite subst_rec_fun_equation. rewrite eq_dec_refl. apply aeq_sub_same.
-        ** apply aeq_refl.
-        ** apply aeq_sym. apply IHt1. assumption.
-      * destruct (atom_fresh (union (fv_nom u) (union (fv_nom (n_sub t1 z t2)) (singleton z')))). simpl in *. apply aeq_sym. rewrite subst_rec_fun_equation. destruct (swap_var x y z' == swap_var x y z).
-        ** apply (swap_neq x y) in n. contradiction.
-        ** destruct (atom_fresh (union (fv_nom (swap x y u)) (union (fv_nom (n_sub (swap x y t1) (swap_var x y z) (swap x y t2))) (singleton (swap_var x y z'))))). case (x1 == (swap_var x y x0)).
-           *** intro Heq. subst. apply aeq_sub_same.
-               **** apply aeq_sym. rewrite <- swap_equivariance. apply H.
-                    ***** reflexivity.
-                    ***** assumption.
-               **** apply aeq_sym. apply IHt1. assumption.
-           *** intro Hneq'. simpl in *. apply aeq_trans with (n_sub (subst_rec_fun (swap x y (swap z x0 t1)) (swap x y u) (swap_var x y z')) (swap_var x y x0) (subst_rec_fun (swap x y t2) (swap x y u) (swap_var x y z'))). 
-               **** apply aeq_sub_diff.
-               ***** apply aeq_refl.
-               ***** assumption.
-               ***** pose proof n2 as Hx1. apply notin_union_2 in n2. apply notin_union_1 in n2. apply notin_union_1 in n2. apply notin_remove_1 in n2. destruct n2.
-               ****** apply fv_nom_remove.
-               ******* apply notin_union_1 in Hx1. assumption.
-               ******* apply notin_remove_2. rewrite swap_equivariance. subst. pose proof n0 as Hx0. apply notin_union_2 in n0. apply notin_union_1 in n0. apply notin_union_1 in n0. apply notin_remove_1 in n0. destruct n0.
-               ******** subst. contradiction.
-               ******** apply fv_nom_swap. apply notin_fv_nom_equivariance. assumption.
-               ****** apply fv_nom_remove.
-               ******* apply notin_union_1 in Hx1. assumption.
-               ******* apply notin_remove_2. rewrite swap_equivariance. apply notin_union_2 in Hx1. apply notin_union_1 in Hx1. apply notin_union_1 in Hx1. apply notin_remove_1 in Hx1. case (swap_var x y z == x1).
-               ******** intro Heq. subst. apply fv_nom_swap. apply notin_union_2 in n0. apply notin_union_1 in n0. apply notin_union_1 in n0. apply notin_remove_1 in n0. destruct n0.
-               ********* subst. contradiction.
-               ********* apply notin_fv_nom_equivariance. assumption.
-               ******** intro Hneq''. destruct Hx1.
-               ********* contradiction.
-               ********* apply fv_nom_remove_swap.
-               ********** assumption.
-               ********** apply aux_not_equal. assumption.
-               ********** assumption.
-               ***** rewrite H.
-               ****** replace (swap_var (swap_var x y x0) x1 (swap_var x y z')) with (swap_var x y z').
-               ******* apply aeq_m_subst_eq.
-               ******** rewrite (swap_equivariance _ x y z x0). apply aeq_sym. rewrite swap_symmetric. rewrite (swap_symmetric _ (swap_var x y z) (swap_var x y x0)). rewrite (swap_symmetric _ (swap_var x y z) x1). pose proof n0 as Hx0. pose proof n2 as Hx1. apply notin_union_2 in n2. apply notin_union_1 in n2. apply notin_union_1 in n2. apply notin_remove_1 in n2. destruct n2.
-               ********* subst. rewrite swap_id. apply notin_union_2 in n0. apply notin_union_1 in n0. apply notin_union_1 in n0. apply notin_remove_1 in n0. case (z == x0).
-               ********** intro Heq. subst. repeat rewrite swap_id. apply aeq_refl.
-               ********** intro Hneq''. rewrite (swap_symmetric _ (swap_var x y z) (swap_var x y x0)). rewrite swap_involutive. apply aeq_refl.
-               ********* apply notin_union_2 in n0. apply notin_union_1 in n0. apply notin_union_1 in n0. apply notin_remove_1 in n0. case (z == x0).
-               ********** intro Heq. subst. rewrite swap_id. apply aeq_refl.
-               ********** intro Hneq''. destruct n0.
-               *********** contradiction.
-               *********** apply aeq_swap_swap.
-               ************ assumption.
-               ************ apply notin_union_2 in Hx0. apply notin_union_1 in Hx0. apply notin_union_1 in Hx0. apply notin_remove_1 in Hx0. destruct Hx0.
-               ************* contradiction.
-               ************* apply notin_fv_nom_equivariance. assumption.
-               ******** symmetry. apply swap_reduction.
-               ********* apply notin_fv_nom_equivariance. apply notin_union_1 in n0. assumption.
-               ********* apply notin_union_1 in n2. assumption.
-               ******* symmetry. unfold swap_var at 1. destruct (swap_var x y z' == swap_var x y x0).
-               ******** repeat apply notin_union_2 in n0. apply notin_singleton_1 in n0. apply (swap_neq x y) in n0. contradiction.
-               ******** destruct (swap_var x y z' == x1).
-               ********* repeat apply notin_union_2 in n2. apply notin_singleton_1 in n2. contradiction.
-               ********* reflexivity.
-               ****** apply swap_size_eq.
-               ****** apply aux_not_equal. assumption.
-               **** apply aeq_sub_same.
-                    ***** apply aeq_sym. apply H.
+                    ********** apply notin_fv_nom_equivariance. assumption. (** The former condition is routine.*)
+                    ***** rewrite H. (** The later condition is proved using the induction hypothesis twice to propagate the swaps inside the metasubstitutions on each side of the $\alpha$-equality. This swap has no effect on the variable of the metasubstitution, therefore we can apply lemma [aeq_m_subst_eq] and each generated case is proved by routine manipulation of swaps.*)
+                    ****** apply aeq_sym. rewrite H.
+                    ******* replace (swap_var x1 (swap_var x y' x0) (swap_var x y' z)) with (swap_var x y' z).
+                    ******** apply aeq_m_subst_eq.
+                    ********* rewrite (swap_symmetric _ x1 (swap_var x y' x0)). rewrite (swap_symmetric _ (swap_var x y' y) x1). case (x0 == y). 
+                    *********** intro Heq. subst. rewrite (swap_symmetric _ (swap_var x y' y) x1). rewrite swap_involutive. rewrite swap_id. apply aeq_refl.
+                    *********** intro Hneq''. rewrite (swap_symmetric _ y x0). rewrite (swap_equivariance _ x y' x0 y). case (x1 == swap_var x y' y). 
+                    ************ intro Heq. subst. rewrite swap_id. apply aeq_refl.
+                    ************ intro Hneq'''. apply aeq_swap_swap.
+                    ************** apply notin_fv_nom_equivariance. apply notin_union_2 in n1. apply notin_union_1 in n1. apply notin_remove_1 in n1. destruct n1.
+                    *************** symmetry in H0. contradiction.
+                    *************** assumption.
+                    ************** apply notin_union_2 in n2. apply notin_union_1 in n2. apply notin_remove_1 in n2. destruct n2.
+                    *************** symmetry in H0. contradiction.
+                    *************** assumption.
+                    ********* apply swap_reduction.
+                    ********** apply notin_union_1 in n2. assumption.
+                    ********** apply notin_union_1 in n1. apply notin_fv_nom_equivariance. assumption.
+                    ******** symmetry. unfold swap_var at 1. destruct (swap_var x y' z ==  x1).
+                    ********* repeat apply notin_union_2 in n2. apply notin_singleton_1 in n2. contradiction.
+                    ********* destruct (swap_var x y' z == swap_var x y' x0).
+                    ********** repeat apply notin_union_2 in n1. apply notin_singleton_1 in n1. apply (swap_neq x y') in n1. contradiction.
+                    ********** reflexivity.
+                    ******* apply swap_size_eq.
+                    ******* assumption.
                     ****** reflexivity.
                     ****** assumption.
-                    ***** apply aeq_sym. apply IHt1. assumption.
-Qed.
-
-(* talvez possa ser substituído pelos lemas parciais anteriores
-Theorem aeq_m_subst: forall t t' u u' x x', x `notin` fv_nom t' -> t =a (swap x x' t') -> u =a u' -> ([x := u] t) =a ([x' := u'] t').
-Proof.
-  intros t t' u u' x x'. case (x == x').
-  - intro Heq; subst. intros Hfv Haeq Haeq'. apply aeq_m_subst_eq.
-    + rewrite swap_id in Haeq. assumption.
-    + assumption.
-  - intros Hneq Hfv Haeq Haeq'. unfold m_subst. apply aeq_trans with (subst_rec_fun (swap x x' t') u x).
-    + apply aeq_m_subst_eq. Admitted.
-(*      * apply (aeq_swap1 _ _ x x') in H1. rewrite H1. rewrite swap_involutive. apply aeq_refl.
-      * apply aeq_refl.
-    + apply aeq_trans with (subst_rec_fun (swap x x' t') u' x).
-      * apply aeq_m_subst_in. assumption.
-      * replace (subst_rec_fun (swap x x' t') u' x) with (subst_rec_fun (swap x x' t') u' (swap_var x x' x')).
-        ** Admitted. (* verificar a estrutura utilizada *) *) *)
-
-(* substituído pelos dois lemas seguintes (corolário)
-Lemma m_subst_abs : forall u x y t , m_subst u x (n_abs y t)  =a
-       if (x == y) then (n_abs y t )
-       else let (z,_) := atom_fresh (fv_nom u `union` fv_nom (n_abs y t ) `union` {{x}}) in
-       n_abs z (m_subst u x (swap y z t )).
-Proof.
-  intros u x y t. destruct (atom_fresh (union (fv_nom u) (union (fv_nom (n_abs y t)) (singleton x)))) as [z H]. destruct (x == y).
-  - subst. unfold m_subst. rewrite subst_rec_fun_equation. rewrite eq_dec_refl. apply aeq_refl.
-  - unfold m_subst. rewrite subst_rec_fun_equation. destruct (x == y).
-    + contradiction.
-    + destruct (atom_fresh (union (fv_nom u) (union (fv_nom t) (union (singleton x) (singleton y))))). case (x0 == z).
-      * intro Heq. subst. Admitted. *)
-
-(*        apply aeq_refl.
-      * intro Hneq. apply aeq_abs_diff.
-        ** assumption.
-        ** apply fv_nom_remove.
-           *** apply notin_union_1 in n1. assumption.
-           *** apply notin_union_2 in H. apply notin_union_1 in H. simpl in H. apply notin_remove_1 in H. destruct H.
-               **** subst. rewrite swap_id. apply notin_remove_2. apply notin_union_2 in n1. apply notin_union_1 in n1. assumption.
-               **** apply notin_remove_2. apply fv_nom_remove_swap.
-                    ***** assumption.
-                    ***** repeat apply notin_union_2 in n1. apply notin_singleton_1 in n1. apply aux_not_equal. assumption.
-                    ***** apply notin_union_2 in n1. apply notin_union_1 in n1. assumption.
-        ** case (y == z).
-           *** intro Heq. subst. rewrite swap_id. apply aeq_trans with (subst_rec_fun (swap z x0 t) (swap z x0 u) (swap_var z x0 x)).
-           **** pose proof aeq_m_subst as H1. unfold m_subst in H1. unfold swap_var. destruct (x == z).
-                ***** repeat apply notin_union_2 in H. apply notin_singleton_1 in H. contradiction.
-                ***** destruct (x == x0).
-                ****** apply notin_union_2 in n1. apply notin_union_2 in n1. apply notin_union_1 in n1. apply notin_singleton_1 in n1. contradiction.
-                ****** apply H1.
-                ******* apply aeq_sym. Admitted. *)
-
-(* apply aeq_refl.
-                ******* Search swap. apply aeq_sym. apply swap_reduction.
-                ******** apply notin_union_1 in H. assumption.
-                ******** apply notin_union_1 in n1. assumption.
-           **** apply aeq_sym. apply swap_subst_rec_fun.
-           *** intro Heq. Search aeq_swap_swap. Search swap. rewrite swap_subst_rec_fun.
-               pose proof aeq_m_subst as H1. unfold m_subst in H1. unfold swap_var. destruct (x == z).
-                **** repeat apply notin_union_2 in H. apply notin_singleton_1 in H. contradiction.
-                **** destruct (x == x0).
-                ***** apply notin_union_2 in n1. apply notin_union_2 in n1. apply notin_union_1 in n1. apply notin_singleton_1 in n1. contradiction.
-                ***** apply H1.
-                ****** apply aeq_sym. Search aeq. rewrite swap_symmetric. pose proof swap_symmetric as H2. specialize (H2 t y z). rewrite H2.
-                       pose proof swap_symmetric as H3. specialize (H3 t y x0). rewrite H3. apply aeq_swap_swap.
-                ******* apply notin_union_2 in n1. apply notin_union_1 in n1. assumption.
-                ******* apply notin_union_2 in H. apply notin_union_1 in H. Search n_abs. simpl in H. Search remove.
-                        apply diff_remove_2 in H.
-                ******** assumption.
-                ******** auto.
-                ****** Search swap. rewrite swap_reduction.
-                ******* apply aeq_refl.
-                ******* apply notin_union_1 in H. assumption. 
-                ******* apply notin_union_1 in n1. assumption. 
-Qed. *)
-
-(** The following lemma states that applying the meta-substitution to the application is equivalent to applying it to eacch term of the application separately. **)
-
-Lemma m_subst_app: forall t1 t2 u x, [x := u](n_app t1 t2) = n_app ([x := u]t1) ([x := u]t2).
-Proof.
-  intros t1 t2 u x. unfold m_subst. rewrite subst_rec_fun_equation. reflexivity.
+    + intros x y H z u. rewrite subst_rec_fun_equation. simpl. apply aeq_sym. rewrite subst_rec_fun_equation. apply aeq_sym. apply aeq_app.
+      * apply IHt2. assumption.
+      * apply IHt1. assumption.
+    + intros x y' Hneq z u. simpl. case (y == z). (** The case of the explicit substitution follows a similar strategy of the abstraction. The initial goal is to prove that [swap x y ([z := u](n_sub t1 y' t2)) =a [(swap_var x y z) := (swap x y u)](swap x y (n_sub t1 y' t2))] and we start comparing the variables [y'] and [z].*)
+      * intro Heq. subst. rewrite subst_rec_fun_equation. apply aeq_sym. rewrite subst_rec_fun_equation. repeat rewrite eq_dec_refl. simpl. apply aeq_sub_same. (** When [y' = z], the metasubstitution has no effect on the body of the metasubstitution but it can still be propagated to the term [t2]. Therefore, this case is proved using the induction hypothesis over [t2]. *)
+        ** apply aeq_refl.
+        ** apply aeq_sym. apply IHt1. assumption.
+      * intro Hneq'. rewrite subst_rec_fun_equation. apply aeq_sym. rewrite subst_rec_fun_equation. destruct (z == y).
+        ** symmetry in e. contradiction.
+        ** destruct (swap_var x y' z == swap_var x y' y).
+           *** apply (swap_neq x y') in n. contradiction.
+           *** destruct (atom_fresh (union (fv_nom u) (union (fv_nom (n_sub t1 y t2)) (singleton z)))). destruct (atom_fresh (union (fv_nom (swap x y' u)) (union (fv_nom (n_sub (swap x y' t1) (swap_var x y' y) (swap x y' t2))) (singleton (swap_var x y' z))))). simpl in *. apply aeq_sym. case (x1 == swap_var x y' x0). (** When [y' <> z], then the metasubstitutions are propagated on both sides of the $\alpha$-equation. Analogously to the abstraction case, one new name for each propagation is necessary. Let [x0] be a new name not in the set $fv(\esub{t1}{y'}{t2})\cup fv(u) \cup \{z\}$, and [x1], a new name not in the set $fv(\esub{\swap{x}{y}{t1}}{\vswap{x}{y}{y'}}{\swap{x}{y}{t2}})\cup fv(\swap{x}{y}{u}) \cup \{\vswap{x}{y}{z}\}$. After the propagation step, we have the goal [n_sub (swap x y ([z := u](swap y' x0 t1))) (swap_var x y x0) (swap x y ([z := u]t2)) =a
+  n_sub ([(swap_var x y z) := (swap x y u)](swap (swap_var x y y') x1 (swap x y t1))) x1
+    ([(swap_var x y z) := (swap x y u)](swap x y t2))]. We proceed by comparing [x1] and [(swap x y x0)].*)
+               **** intro Heq. subst. apply aeq_sub_same. (** If [x1 = swap_var x y x0] then after an application of the rule [aeq_sub_same], each component of the explicit substitution is proved by the induction hypothesis.*)
+                    ***** rewrite <- swap_equivariance. apply H.
+                    ****** reflexivity.
+                    ****** assumption.
+                    ***** apply IHt1. assumption.
+               **** intro Hneq''. apply aeq_sub_diff.
+                    ***** apply IHt1. assumption. (** If [x1 <> swap_var x y x0] then we apply the rule [aeq_sub_diff] to decompose the explicit substitution in its components. The second component is straightforward  by the induction hypothesis.*)
+                    ***** apply aux_not_equal. assumption.
+                    ***** apply fv_nom_remove.
+                    ****** apply notin_fv_nom_equivariance. apply notin_union_1 in n1. assumption.
+                    ****** apply notin_remove_2. case (y == x0).
+                    ******* intro Heq. subst. apply fv_nom_swap. apply notin_union_2 in n2. apply notin_union_1 in n2. apply notin_union_1 in n2. apply notin_remove_1 in n2. destruct n2.
+                    ******** symmetry in H0. contradiction.
+                    ******** assumption.
+                    ******* intro Hneq'''. apply fv_nom_remove_swap.
+                    ******** apply aux_not_equal. assumption.
+                    ******** apply (swap_neq x y') in Hneq'''. apply aux_not_equal. assumption.
+                    ******** apply notin_fv_nom_equivariance. apply notin_union_2 in n1. apply notin_union_1 in n1. apply notin_union_1 in n1. apply notin_remove_1 in n1. destruct n1.
+                    ********* contradiction.
+                    ********* assumption.
+                    ***** rewrite H. (** The first component follows the strategy used in the abstraction case. The current goal, obtained after the application of the rule [aeq_sub_diff] is [swap x y ([z := u](swap y' x0 t1)) =a
+  swap x1 (swap_var x y x0) ([(swap_var x y z) := (swap x y u)](swap (swap_var x y y') x1 (swap x y t1)))]. The induction hypothesis is used twice to propagate the swap on both the LHS and RHS of the $\alpha$-equality. This swap has no effect on the variable of the metasubstitution, therefore we can apply lemma [aeq_m_subst_eq] and each generated case is proved by routine manipulation of swaps. $\hfill\Box$*)
+                    ****** apply aeq_sym. rewrite H.
+                    ******* replace (swap_var x1 (swap_var x y' x0) (swap_var x y' z)) with (swap_var x y' z).
+                    ******** apply aeq_m_subst_eq.
+                    ********* rewrite (swap_symmetric _ x1 (swap_var x y' x0)). rewrite (swap_symmetric _ (swap_var x y' y) x1). case (x0 == y). 
+                    *********** intro Heq. subst. rewrite (swap_symmetric _ (swap_var x y' y) x1). rewrite swap_involutive. rewrite swap_id. apply aeq_refl.
+                    *********** intro Hneq'''. rewrite (swap_symmetric _ y x0). rewrite (swap_equivariance _ x y' x0 y). case (x1 == swap_var x y' y). 
+                    ************ intro Heq. subst. rewrite swap_id. apply aeq_refl.
+                    ************ intro Hneq''''. apply aeq_swap_swap.
+                    ************** apply notin_fv_nom_equivariance. apply notin_union_2 in n1. apply notin_union_1 in n1. apply notin_union_1 in n1. apply notin_remove_1 in n1. destruct n1.
+                    *************** symmetry in H0. contradiction.
+                    *************** assumption.
+                    ************** apply notin_union_2 in n2. apply notin_union_1 in n2. apply notin_union_1 in n2. apply notin_remove_1 in n2. destruct n2.
+                    *************** symmetry in H0. contradiction.
+                    *************** assumption.
+                    ********* apply swap_reduction.
+                    ********** apply notin_union_1 in n2. assumption.
+                    ********** apply notin_union_1 in n1. apply notin_fv_nom_equivariance. assumption.
+                    ******** symmetry. unfold swap_var at 1. destruct (swap_var x y' z ==  x1).
+                    ********* repeat apply notin_union_2 in n2. apply notin_singleton_1 in n2. contradiction.
+                    ********* destruct (swap_var x y' z == swap_var x y' x0).
+                    ********** repeat apply notin_union_2 in n1. apply notin_singleton_1 in n1. apply (swap_neq x y') in n1. contradiction.
+                    ********** reflexivity.
+                    ******* apply swap_size_eq.
+                    ******* assumption.
+                    ****** reflexivity.
+                    ****** assumption.
 Qed.
 
 (* begin hide *)
-
 Lemma m_subst_abs: forall t1 u x y, [x := u](n_abs y t1)  =a
        if (x == y) then (n_abs y t1)
        else let (z,_) := atom_fresh (fv_nom u `union` fv_nom (n_abs y t1) `union` {{x}}) in n_abs z (subst_rec_fun (swap y z t1) u x).
@@ -2913,9 +2176,7 @@ Proof.
 Qed.
 (* end hide *)
 
-(** The following lemmas state, respectively, what hapens when the variable in the meta-substitution is equal or different from the one in the abstraction. When it is equal, the meta-substitution is irrelevant. When they are different, we take a new variable that does not occur freely in the substituted term in the meta-substitution nor in the abstraction and is not the variable in the meta-substitution, and the abstraction of this new variable using the meta-substitution of the swap of the former variable in the meta-substitution is alpha-equivalent to the original meta-substitution of the abstraction. **)
-(** The proofs were made using the definition of the meta-substitution, each case being respectively each one in the definition.**)
-
+(** The following lemmas state, respectively, what hapens when the variable in the meta-substitution is equal or different from the one in the abstraction. When it is equal, the meta-substitution is irrelevant. When they are different, we take a new variable that does not occur freely in the substituted term in the meta-substitution nor in the abstraction and is not the variable in the meta-substitution, and the abstraction of this new variable using the meta-substitution of the swap of the former variable in the meta-substitution is alpha-equivalent to the original meta-substitution of the abstraction. The proofs were straightforward from the definition of the meta-substitution, each case being respectively each one in the definition. %\newline%*)
 Lemma m_subst_abs_eq : forall u x t, [x := u](n_abs x t) = n_abs x t.
 Proof.
   intros u x t. unfold m_subst. rewrite subst_rec_fun_equation. rewrite eq_dec_refl. reflexivity.
@@ -2966,7 +2227,6 @@ Proof.
 Qed.
 
 (* begin hide *)
-
 Lemma m_subst_sub: forall t1 t2 u x y, [x := u](n_sub t1 y t2)  =a
        if (x == y) then (n_sub t1 y ([x := u]t2))
        else let (z,_) := atom_fresh (fv_nom u `union` fv_nom (n_sub t1 y t2) `union` {{x}}) in
@@ -2978,11 +2238,9 @@ Proof.
     + simpl. contradiction.
     + simpl. destruct (atom_fresh (union (fv_nom u) (union (fv_nom (n_sub t1 y t2)) (singleton x)))). apply aeq_refl.
 Qed.
-
 (* end hide *)
 
-(** The following lemmas state, respectively, what hapens when the variable in the meta-substitution is equal or different from the one in the explicit substitution. When it is equal, the meta-substitution is irrelevant on [t1], but it is applied to [e2]. When they are different, we take a new variable that does not occur freely in the substituted term in the meta-substitution nor in the substitution and is not the variable in the meta-substitution, and the explicit substitution of this new variable using the meta-substitution of the swap of the former variable in the meta-substitution in [e11] and the application of the original meta_substitution in [e12] is alpha-equivalent to the original meta-substitution of the explicit substitution. **)
-(** The proofs were made using the definition of the meta-substitution, each case being respectively each one in the definition.**)
+(** The following lemmas are the equivalent version of the two previous lemmas for the case of the explicit substitution. They state, respectively, what hapens when the variable in the meta-substitution is equal or different from the one in the explicit substitution. When it is equal, the meta-substitution is irrelevant on [t1], but it is applied to [e2]. When they are different, we take a new variable that does not occur freely in the substituted term in the meta-substitution nor in the substitution and is not the variable in the meta-substitution, and the explicit substitution of this new variable using the meta-substitution of the swap of the former variable in the meta-substitution in [e11] and the application of the original meta_substitution in [e12] is alpha-equivalent to the original meta-substitution of the explicit substitution. The proofs are straighforward from the definition of the meta-substitution, each case being respectively each one in the definition. %\newline%*)
 
 Lemma m_subst_sub_eq : forall u x t1 t2, [x := u](n_sub t1 x t2) = n_sub t1 x ([x := u] t2).
 Proof.
@@ -3031,143 +2289,15 @@ Proof.
                **** subst. repeat apply notin_union_2 in n0. apply notin_singleton_1 in n0. contradiction.
                **** reflexivity.
 Qed.
-
-(*       unfold swap_var. destruct (x == z).
-        ** subst. apply notin_union_2 in H2. apply notin_union_2 in H2. apply notin_singleton_1 in H2. contradiction.
-        ** destruct (x == x0).
-           *** subst. repeat apply notin_union_2 in n0. apply notin_singleton_1 in n0. contradiction.
-           *** pose proof aeq_m_subst_eq as Heq. unfold m_subst in *. apply Heq.
-               **** rewrite swap_symmetric. apply aeq_sym. rewrite swap_symmetric. pose proof swap_symmetric as Hswap. specialize (Hswap t1 y z).
-                    rewrite Hswap. apply aeq_swap_swap.
-                    ***** destruct (x0 == y).
-                          ****** subst. apply notin_union_2 in n0. apply notin_union_1 in n0. simpl in n0. apply remove_notin in n0.  assumption.
-                          ****** apply notin_union_2 in n0. apply notin_union_1 in n0. simpl in n0. apply diff_remove_2 in n0; assumption.
-                    ***** apply notin_union_2 in H2. apply notin_union_1 in H2. destruct (z == y).
-                          ****** subst. apply remove_notin in H2. assumption.
-                          ****** simpl in H2. apply diff_remove_2 in H2; assumption.                    
-               **** apply aeq_sym. apply swap_reduction.
-                    ***** apply notin_union_1 in H2. assumption.
-                    ***** apply notin_union_1 in n0. assumption.
-Qed. *)
-
-(*    destruct (atom_fresh (union (fv_nom u) (union (fv_nom t) (union (singleton x) (singleton y))))). case (x0 == z) eqn: H.
-    + subst. apply aeq_abs_same. apply aeq_refl.
-    + apply aeq_abs_diff.
-      * assumption.
-      * admit.
-      * apply aeq_sym. rewrite swap_subst_rec_fun_out.
-        
-    induction t using n_sexp_induction.
-  - intros u x' y z H1 H2. sim
-  intros u x y z t H H1. pose proof m_subst_abs as H2. specialize (H2 u x y t). destruct (x == y) eqn:Hx.
-  - subst. contradiction.
-  - destruct (atom_fresh (Metatheory.union (fv_nom u) (Metatheory.union (fv_nom (n_abs y t)) (singleton x)))).
-    apply aeq_trans with (n_abs x0 ([x := u] swap y x0 t)).
-    + assumption.
-    + case (x0 == z).
-      * intro H3. rewrite H3. apply aeq_refl.
-      * intro H3. simpl in *. Search n_abs. admit. (*rewrite test1. rewrite test1. Search n_abs. apply aeq_abs_diff.
-        ** auto.
-        ** admit.
-        ** apply test2.*)
- *) 
-
-
-(*
-Corollary m_subst_abs_neq : forall u x y t, x <> y -> let (z,_) := atom_fresh (fv_nom u `union` fv_nom (n_abs y t ) `union` {{x}}) in [x := u](n_abs y t) =a n_abs z ([x := u](swap y z t)).
-Proof.
-  intros u x y t H. pose proof m_subst_abs. specialize (H0 u x y t). destruct (x == y) eqn:Hx.
-  - subst. contradiction.
-  - destruct (atom_fresh (Metatheory.union (fv_nom u) (Metatheory.union (fv_nom (n_abs y t)) (singleton x)))). assumption.    
-Qed.  
-*)
-  
-(*Lemma m_subst_abs_diff : forall t u x y, x <> y -> x `notin` (remove y (fv_nom t)) -> [x := u](n_abs y t) = n_abs y t.
-Proof. 
-  intros t u x y H0 H1. Search n_abs. admit.
-
-  *)
  
 (** * The substitution lemma for the metasubstitution *)
 
-(**
-   In the pure $\lambda$-calculus, the substitution lemma is probably the first non trivial property. In our framework, we have defined two different substitution operation, namely, the metasubstitution denoted by [[x:=u]t] and the explicit substitution that has [n_sub] as a constructor. In what follows, we present the main steps of our proof of the substitution lemma for the metasubstitution operation: 
- *)
+(** In the pure $\lambda$-calculus, the substitution lemma is probably the first non trivial property. In our framework, we have defined two different substitution operation, namely, the metasubstitution denoted by [[x:=u]t] and the explicit substitution that has [n_sub] as a constructor. In what follows, we present the main steps of our proof of the substitution lemma for the metasubstitution operation: *)
 
-
-Lemma m_subst_lemma: forall e1 e2 x e3 y, x <> y -> x `notin` (fv_nom e3) ->
- ([y := e3]([x := e2]e1)) =a ([x := ([y := e3]e2)]([y := e3]e1)).
+Lemma m_subst_lemma: forall e1 e2 x e3 y, x <> y -> x `notin` (fv_nom e3) -> ([y := e3]([x := e2]e1)) =a ([x := ([y := e3]e2)]([y := e3]e1)).
 Proof.
-
-(* Due to permutation propagation, a stronger induction hypothesis is needed.
-  (** We proceed by functional induction on the structure of function [subst_rec_fun], i.e. the definition of the meta-substitution. The induction splits the proof in seven cases: two cases concern variables, the next two concern abstractions, the next case concerns the application and the last two concern the explicit substitution.  *) 
-  intros e1 e2 x. functional induction (subst_rec_fun e1 e2 x).
-  (** *)
-  (**The first case is about the variable. It considers that there are two variables, $x$ and $y$ and they differ from one another. *)
-  - intros e3 y XY H. rewrite m_subst_var_eq. rewrite m_subst_var_neq.
-  (** *)
-  (**When we rewrite the lemmas concerning equality and negation on variables substitution, we have two cases.*)
-  (** *)
-  (**If we only have these two variables, we can use the equality lemma to find that both sides of the proof are equal and finish it using reflexivity and in the second case assumptions are used to finish the proof.*)
-    + rewrite m_subst_var_eq. apply aeq_refl.
-    + assumption.
-  (** *)
-  (**The second case is also about variables. In it, we consider a third variable, $z$, meaning that each variable is different from the other. In the former case, we had that $x = y$.*)
-  - intros e3 z XY H. rewrite m_subst_var_neq.
-  (** *)
-  (**To unfold the cases in this proof, we need to destruct one variable as another. We chose to do $x == z$.*)
-    + destruct (y == z) eqn:Hyz.
-  (** *)
-  (**This splits the proof in two cases.*)
-  (** *)
-  (**In the first case, we have that $x = z$. To expand this case, we use the lemma $m_subst_notin$ as an auxiliary lemma. It is added as an hypothesis, using the specialization tactics to match the last case in that hypothesis to the proof we want.*)
-  (** *)
-(*   (**The rest of the caases are finished  using the varible substitution's negation of equality, the varible substitution's equality or the standard library lemmas.*)  *)
-    * subst. rewrite m_subst_var_eq. pose proof m_subst_notin as H'. specialize (H' e3 ([z := e3] u) x). apply aeq_sym. apply H'; assumption.
-      * rewrite m_subst_var_neq.
-        ** rewrite m_subst_var_neq.
-           *** apply aeq_refl.
-           *** auto.
-        ** auto.
-    + auto. 
-  - intros e3 z XY H. rewrite m_subst_abs_eq.
-    pose proof m_subst_notin as H'. specialize (H' ([z := e3] n_abs x t1) ([z := e3] u) x). 
-    apply aeq_sym. apply H'. apply fv_nom_remove.
-    + assumption.
-    + apply diff_remove.
-      * assumption.
-      * simpl. apply notin_remove_3. reflexivity.
-  - intros e3 y' XY H. destruct (y == y').
-    + subst. rewrite m_subst_abs_eq. rewrite m_subst_notin_m_subst.
-      * apply aeq_refl.
-      * simpl. apply notin_remove_3. reflexivity.
-    + rewrite m_subst_abs_neq.
-      unfold m_subst in *. specialize (IHn e3 y'). admit. 
-(*
-      pose proof m_subst_abs_neq. specialize (H u x y t1). destruct (atom_fresh (union (fv_nom u) (union (fv_nom (n_abs y t1)) (singleton x)))). clear e0. assert (Hxy := _x). apply H in _x. rewrite _x. clear H.
-      * destruct (x0 == y').
-        ** pose proof m_subst_abs_neq. specialize (H e3 y' y t1). destruct (atom_fresh (union (fv_nom e3) (union (fv_nom (n_abs y t1)) (singleton y')))). rewrite H.
-           ***
-           ***
-          subst. rewrite m_subst_abs_eq.
-        **
-      * *)
-  (** *)
-  (**The case of application is solved by using the auxiliary lemmas on application. First, it is rewritten so that the substitution is made inside the aplication, instead of on it. The same lemma is applied multiple times to make sure nothing can be replaced anymore. This leads to a case that can be solved using the standard library lemmas.*)
-  - intros e3 z XY IH. rewrite m_subst_app. rewrite m_subst_app. rewrite m_subst_app.  rewrite m_subst_app. auto.
-  - intros e3 z XY IH.  admit.
-  - admit.  *)
-
-
-(*  induction e1 using n_sexp_size_induction. *) 
-
-  (** We procced by case analisys on the structure of [e1]. The cases in between square brackets below mean that in the first case, [e1] is a variable named [z], in the second case [e1] is an abstraction of the form $\lambda$[z.e11], in the third case [e1] is an application of the form ([e11] [e12]), and finally in the fourth case [e1] is an explicit substitution of the form [e11] $\langle$ [z] := [e12] $\rangle$. *)
-  
-  induction e1 using n_sexp_induction.
-
-  (** The variable case was proved using the auxiliary lemmas on the equality and inequality of the meta-substitution applied to variables. It was also necessary to compare the variable in the meta-substitution and the variable one in each case of this proof.**)
-
-  - (* variable case: *) intros e2 x' e3 y Hneq Hfv. case (x == x').
+  induction e1 using n_sexp_induction. (** %\noindent{\bf Proof.}% The proof is by induction on the size of the term [e1]. The interesting cases are the abstraction and the explicit substitution.*)
+- intros e2 x' e3 y Hneq Hfv. case (x == x').
     + intro Heq. subst. rewrite m_subst_var_eq. case (x' == y).
       * intro Heq. subst. contradiction.
       * intro Hneq'. rewrite m_subst_var_neq.
@@ -3188,29 +2318,25 @@ Proof.
                **** assumption.
            *** assumption.
         ** assumption.
-
-      (** In the abstraction case, we used a similar approach, comparing the variable in the meta substitution and the one in the abstraction. When usion the using the auxiliary lemmas on the equality and inequality of the meta-substitution applied to abstractions, it was necessary to create new variables in each use of the inequality. This is due to the atempt of removing the abstraction from inside the meta-substitution.**)
-
-  - intros e2 x e3 y Hxy Hfv. case (z == x).
-    + intro Heq. subst. rewrite m_subst_abs_eq. assert (Haeq : ([x := [y := e3] e2] ([y := e3] n_abs x e1)) =a ([y := e3] n_abs x e1)).
-      * apply m_subst_notin. apply fv_nom_remove.
-        ** assumption.
-        ** apply notin_remove_2. simpl. apply notin_remove_3. reflexivity.
-      * apply aeq_sym. auto.
-    + intro Hneq. destruct (y == z).
+  - intros e2 x e3 y Hxy Hfv. case (z == x). (** In the abstraction case, the initial goal is [([y := e3] ([x := e2] n_abs z e1)) =a ([x := [y := e3] e2] ([y := e3] n_abs z e1))], assuming that [x <> y] and [x `notin` fv_nom e3]. The induction hypothesis generated by this case states that the lemma can be propagated to a swap inside a metasubstitution that is applied to a term thath has the same size as [e1] and the same hypothesis for the main lemma also apply to this case. We start comparing [z] with [x] aiming to apply the definition of the metasubstitution on the LHS of the goal.*)
+    + intro Heq. subst. rewrite m_subst_abs_eq. apply aeq_sym. apply m_subst_notin. apply fv_nom_remove. (** When [z = x], the subterm [[x := e2](n_abs x e1)] is reduced to [(n_abs x e1)] by applying the lemma in m_subst_abs_eq and then the LHS reduces to [([y := e3] n_abs x e1)]. The RHS reduces to [([y := e3] n_abs x e1)] because [x] does not occur free neither in [(n_abs x e1)] nor in [e3], which has also been proved.*)
+        * assumption.
+        * apply notin_remove_2. simpl. apply notin_remove_3. reflexivity.
+    + intro Hneq. destruct (y == z). (* When [z <> x], then we compare [y] with [z].*)
       * subst. rewrite m_subst_abs_eq. pose proof m_subst_abs_neq as Habs. pick fresh w for (union (fv_nom e3) (union (fv_nom e2) (union (fv_nom (n_abs z e1)) (singleton x)))). specialize (Habs e1 e2 x z w).
-        apply aeq_trans with ([z := e3] n_abs w ([x := e2] swap z w e1)). apply aeq_m_subst_out.
-        ** apply Habs.
+        apply aeq_trans with ([z := e3] n_abs w ([x := e2] swap z w e1)). 
+        ** apply aeq_m_subst_out. (** When [y = z] then the subterm [([y := e3] n_abs z e1)] reduces to [(n_abs z e1)], by applying the lemma m_subst_abs_neq which also generates certain hypothesis that help prove this fact. On the LHS, we propagate the internal metasubstitution over the abstraction taking a fresh name for the binder that is necessary because of the hypothesys generated using the lemma m_subst_abs_neq as explained previously. Let [w] be a new name that is not in the set $fv(\lambda_z'.e_1) \cup fv(e3) \cup fv(e2) \cup \{x\}$. The resulting terms are $\alpha$-equivalent, and although the strategy is similar to the one used in the lemmas [aeq_m_subst_in], [aeq_m_subst_out] and [swap_subst_rec_fun] the proof requires much more steps. First, we apply the transitivity of the $\alpha$-equivalency using ([z := e3] n_abs w ([x := e2] swap z w e1)) as intermediate term. The first case is the $\alpha$-equivalency of LHS with this new term, wich is solved by applying aeq_m_subst_out trivially. **)
+           apply Habs.
            *** assumption.
            *** apply notin_union_2 in Fr. assumption.
-        ** destruct (z == w).
-           *** subst. rewrite m_subst_abs_eq. rewrite swap_id. pose proof m_subst_abs_neq as Habs'. specialize (Habs' e1 ([w := e3] e2) x w w).
+        ** destruct (z == w). (** The other case is the $\alpha$-equivalency of RHS with this new term. In this case it was necessary to compare other two pairs of variables. Initially, we compared [z] and [w].*)
+           *** subst. rewrite m_subst_abs_eq. rewrite swap_id. pose proof m_subst_abs_neq as Habs'. specialize (Habs' e1 ([w := e3] e2) x w w).  (** When [z = w] then in the LHS the metasubstitution is removed using the lemma [m_subst_abs_eq] and the subterm [([w := e2] swap w w e1)] is reduced to [([w := e2]) e1], remaining only [n_abs w ([x := e2] e1)]. On the RHS, we propagate the internal metasubstitution over the abstraction taking the [w] as the new variable for this substitution. Then, the lemma [aeq_abs_same] is used to remove the abstractions on both sides of the $\alpha$-equivalency and because they have the same variable, all we have to do is assure that the expressions are $\alpha$-equivalent. By applying the lemma [aeq_m_subst_in], we can see that they are. **)
                rewrite Habs'. apply aeq_abs_same. rewrite swap_id. apply aeq_sym. apply aeq_m_subst_in. apply m_subst_notin. apply notin_union_2 in Fr. apply notin_union_1 in Fr. assumption.
                assumption. apply notin_union. apply fv_nom_remove. apply notin_union_1 in Fr. assumption. apply notin_remove_3. reflexivity. apply notin_union_2 in Fr. 
                apply notin_union_2 in Fr. assumption.
-           *** pose proof m_subst_abs_neq as Habs'. specialize (Habs' e1 ([z := e3] e2) x z w). pick fresh w' for (union (fv_nom e3) (union (fv_nom e2) (union (fv_nom (n_abs z e1)) (singleton x)))).
+           *** pose proof m_subst_abs_neq as Habs'. specialize (Habs' e1 ([z := e3] e2) x z w). pick fresh w' for (union (fv_nom e3) (union (fv_nom e2) (union (fv_nom (n_abs z e1)) (singleton x)))). (** In the last part of this case, we propagate the internal metasubstitution over the abstraction taking a fresh name for the binder that is necessary because of the hypothesys generated using the lemma m_subst_abs_neq as explained previously. Let [w'] be a new name that is not in the set $fv(\lambda_z'.e_1) \cup fv(e3) \cup fv(e2) \cup \{x\}$. We then proceed by comparing [w] and [w'].**)
                destruct (w == w'). 
-               **** subst. rewrite Habs'. pose proof m_subst_abs_neq as Habs''. specialize (Habs'' ([x := e2] swap z w' e1) e3 z w' w'). rewrite Habs''.
+               **** subst. rewrite Habs'. pose proof m_subst_abs_neq as Habs''. specialize (Habs'' ([x := e2] swap z w' e1) e3 z w' w'). rewrite Habs''. (** When [w == w'], the proof if given by removing the abstractions from inside the metasubstitutions using the lemma [m_subst_abs_neq] and the new variable [w']. Then we remove them altogether using the lemma [aeq_abs_same], given that the variables in the abstractions are the same. The subterm [swap w' w' ([x := e2] swap z w' e1)] gets simplified to [([x := e2] swap z w' e1)], in the LHS. What remain is simmilar to what we have in our induction hypothesys, which is applied to our conclusion and the rest of the proof is solved trivially. The case in which [w <> w'] is solved similarly.**)
                     apply aeq_abs_same. rewrite swap_id. rewrite H. apply aeq_m_subst_out. apply m_subst_notin. apply fv_nom_swap. apply notin_union_2 in Fr. apply notin_union_2 in Fr.
                     apply notin_union_1 in Fr. simpl in *. apply diff_remove_2 in Fr. assumption. apply not_eq_sym. assumption. reflexivity. assumption. assumption.
                     assumption. apply notin_union. apply notin_union_1 in Fr. assumption. apply notin_union. simpl. apply notin_remove_3. reflexivity. apply notin_singleton_2. assumption.
@@ -3419,17 +2545,11 @@ Proof.
                ***** apply notin_union.
                ****** apply notin_union_2 in Fr. apply notin_union_2 in Fr. apply notin_union_1 in Fr. assumption.
                ****** repeat apply notin_union_2 in Fr. assumption.  
-
-    (** The case of the application is simple to solve. It consisted of applying the auxiliary lemma of removing the application from inside the meta-substitution. **)
-
   - intros e2 x e3 y Hneq Hfv. repeat rewrite m_subst_app. pose proof aeq_app as H. specialize (H ([y := e3] ([x := e2] e1_1)) ([y := e3] ([x := e2] e1_2)) ([x := [y := e3] e2] ([y := e3] e1_1)) ([x := [y := e3] e2] ([y := e3] e1_2))). rewrite H. 
     + apply aeq_refl.
     + apply IHe1_1; assumption.
     + apply IHe1_2; assumption.
-
-      (** In the explicit substitution case, we used the same approach used in the abstraction for the left side and the same as the application for the right side of the substitution. It consisted of comparing the variable in the meta substitution and the one in the substitution. We used the auxiliary lemmas on the equality and inequality of the meta-substitution applied to explicit substitutions and it was necessary to create new variables in each use of the inequality. This is due to the atempt of removing the explicit substitution from inside the meta-substitution. When tis removal was made, the proof consisted in proving a similar case for the abstraction in the left side of the explicit substitution and the one similar to the application was used for the right part of it.**)
-
-  - intros e2 x e3 y Hneq Hfv. case (z == x).
+  - intros e2 x e3 y Hneq Hfv. case (z == x). (** In the explicit substitution case, we used the same approach used in the abstraction for the left side and the same as the application for the right side of the substitution. It consisted of comparing the variable in the meta substitution and the one in the substitution. We used the auxiliary lemmas on the equality and inequality of the meta-substitution applied to explicit substitutions and it was necessary to create new variables in each use of the inequality. This is due to the atempt of removing the explicit substitution from inside the meta-substitution. When tis removal was made, the proof consisted in proving a similar case for the abstraction in the left side of the explicit substitution and the one similar to the application was used for the right part of it.$\hfill\Box$*)
     + intro Heq. subst. rewrite m_subst_sub_eq. assert (Haeq: ([y := e3] n_sub e1_1 x ([x := e2] e1_2)) =a ([x := [y := e3] e2] ([y := e3] n_sub e1_1 x e1_2))).
       * pose proof m_subst_sub_neq as Hsubneq. pick fresh w for (union (fv_nom (n_sub e1_1 x e1_2)) (union (fv_nom e2) (union (fv_nom e3) (union (singleton x) (singleton y))))).
         specialize (Hsubneq e1_1 ([x := e2] e1_2) e3 y x w). pose proof Hneq as H'. apply not_eq_sym in H'. apply Hsubneq in H'. rewrite H'.
@@ -3784,3 +2904,11 @@ Proof.
                ****** apply notin_union_2 in Fr. apply notin_union_2 in Fr. apply notin_union_1 in Fr. assumption.
                ****** repeat apply notin_union_2 in Fr. assumption.  
  Qed.
+
+(** * Conclusion and Future work*)
+
+(** In this work, we presented a formalization of the substitution lemma in a framework that extends the $\lambda$-calculus with an explicit substitution operator. Calculi with explicit substitutions are important frameworks to study properties of the $\lambda$-calculus and have been extensively studied in the last decades%\cite{abadiExplicitSubstitutions1991,accattoliAbstractFactorizationTheorem2012,ayala-rinconComparingCalculiExplicit2002,ayala-rinconComparingImplementingCalculi2005,bonelliPerpetualityNamedLambda2001,fujitaChurchRosserTheoremCompositional2016}%. 
+ 
+The formalization is modular in the sense that the explicit substitution operator is generic and could be instantiated with any calculi with  explicit substitutions in a nominal setting. The main contribution of this work, besides the formalization itself, is the solution to a circular proof problem. Several auxiliary (minor) results were not included in this document, but they are numerous and can be found in the source file of the formalization that is available in a GitHub repository from the following url %\url{https://github.com/flaviodemoura/lx_confl/tree/m_subst_lemma}%.
+
+As future work, we plan to integrate this formalization with another one related to the Z property %\cite{fmm2021}% to prove properties of calculi with explicit substitutions such as confluence%\cite{nakazawaCompositionalConfluenceProofs2016,nakazawaCallbyvalue2017,kesnerPerpetualityFullSafe2008}%. *)
